Wrote up two, mostly finished reproving correctness

06TreeCode/TailCallOptimization.thy
@@ -1,5 +1,5 @@
 theory TailCallOptimization
-  imports TreeCode "../00Utils/Iteration"
+  imports TreeCodeConversion "../00Utils/Iteration"
 begin
 
 subsection \<open>Tail-Call Optimization\<close>
@@ -19,39 +19,52 @@ instruction to express.\<close>
 
 text \<open>What exactly do we change with tail-call optimization? We replace every sequence of an
 \<open>Apply\<^sub>e\<close> followed by a \<open>Return\<^sub>e\<close> with a \<open>Jump\<^sub>e\<close>, obviously. But we also eliminate certain frames from
-the call stack; specifically, any frame that consists of an empty codeblock followed by a \<open>Return\<^sub>e\<close>.
-We mark these frames as \<open>dead_frame\<close>s.\<close>
+the call stack; specifically, any frame that consists nothing but a single \<open>Return\<^sub>e\<close>. We mark these 
+frames as \<open>dead_frame\<close>s.\<close>
 
-fun dead_frame :: "frame\<^sub>e \<Rightarrow> bool" where
-  "dead_frame (\<V>, [], Return\<^sub>e) = True"
-| "dead_frame (\<V>, [], Jump\<^sub>e) = False"
-| "dead_frame (\<V>, op # \<C>, r) = False"
+primrec dead_frame :: "frame\<^sub>e \<Rightarrow> bool" where
+  "dead_frame (\<V>, \<C>) = (\<C> = [Return\<^sub>e])"
 
-text \<open>The optimization itself is simple: we convert the code and returns, then map the conversion up 
-through the levels of the state, taking care to eliminate the dead frames in the stack:\<close>
-
-primrec tco_return :: "code\<^sub>e list \<Rightarrow> return\<^sub>e \<Rightarrow> return\<^sub>e" where
-  "tco_return [] r = r"
-| "tco_return (op # cd) r = (if op = Apply\<^sub>e \<and> cd = [] then Jump\<^sub>e else tco_return cd r)"
+text \<open>The optimization itself is simple: we convert the code, eliminating \<open>Apply\<^sub>e; Return\<^sub>e\<close>s, then 
+map the conversion up through the levels of the state, taking care to also eliminate the dead frames 
+in the stack:\<close>
 
 fun tco_code :: "code\<^sub>e list \<Rightarrow> code\<^sub>e list" where
   "tco_code [] = []"
-| "tco_code (Apply\<^sub>e # []) = []"
-| "tco_code (PushLam\<^sub>e \<C>' r # \<C>) = PushLam\<^sub>e (tco_code \<C>') (tco_return \<C>' r) # tco_code \<C>"
+| "tco_code (Apply\<^sub>e # Return\<^sub>e # \<C>) = Jump\<^sub>e # tco_code \<C>"
+| "tco_code (PushLam\<^sub>e \<C>' # \<C>) = PushLam\<^sub>e (tco_code \<C>') # tco_code \<C>"
 | "tco_code (op # \<C>) = op # tco_code \<C>"
 
 primrec tco_val :: "closure\<^sub>e \<Rightarrow> closure\<^sub>e" where
   "tco_val (Const\<^sub>e n) = Const\<^sub>e n"
-| "tco_val (Lam\<^sub>e \<Delta> \<C> r) = Lam\<^sub>e (map tco_val \<Delta>) (tco_code \<C>) (tco_return \<C> r)"
+| "tco_val (Lam\<^sub>e \<Delta> \<C>) = Lam\<^sub>e (map tco_val \<Delta>) (tco_code \<C>)"
 
 fun tco_frame :: "frame\<^sub>e \<Rightarrow> frame\<^sub>e" where
-  "tco_frame (\<Delta>, \<C>, r) = (map tco_val \<Delta>, tco_code \<C>, tco_return \<C> r)"
+  "tco_frame (\<Delta>, \<C>) = (map tco_val \<Delta>, tco_code \<C>)"
 
 abbreviation tco_stack :: "frame\<^sub>e list \<Rightarrow> frame\<^sub>e list" where
   "tco_stack s \<equiv> filter (\<lambda>f. \<not> dead_frame f) (map tco_frame s)"
 
 primrec tco_state :: "state\<^sub>e \<Rightarrow> state\<^sub>e" where
   "tco_state (S\<^sub>e \<V> s) = S\<^sub>e (map tco_val \<V>) (tco_stack s)"
+
+lemma tco_to_empty [simp]: "(tco_code \<C> = []) = (\<C> = [])"
+  by (induction \<C> rule: tco_code.induct) simp_all
+
+lemma tco_to_return [simp]: "(tco_code \<C> = [Return\<^sub>e]) = (\<C> = [Return\<^sub>e])"
+  by (induction \<C> rule: tco_code.induct) simp_all
+
+lemma tco_to_dead_frame [simp]: "dead_frame (\<Delta>, tco_code \<C>) = (\<C> = [Return\<^sub>e])"
+  by (induction \<C> rule: tco_code.induct) simp_all
+
+lemma tco_frame_to_dead_frame [simp]: "dead_frame (tco_frame f) = dead_frame f"
+  by (induction f) simp_all
+
+lemma tco_to_dead_frame_apply [simp]: "dead_frame (map tco_val \<Delta>, tco_code (Apply\<^sub>e # \<C>)) = False"
+proof (induction \<C> rule: tco_code.induct)
+  case ("4_3" \<C>)
+  thus ?case by (cases \<C>) simp_all
+qed simp_all
 
 text \<open>We will of course prove that tail-call removal is semantics-preserving, but we will not 
 formally prove that it really is "an optimization". Instead, we will prove some much simpler results 
@@ -82,23 +95,39 @@ express that no \<open>PushLam\<^sub>e\<close> contains code for a dead frame, a
 always be the case, pre-optimization).\<close>
 
 fun complete_lams :: "code\<^sub>e list \<Rightarrow> bool" where
-  "complete_lams [] = True"
-| "complete_lams (PushLam\<^sub>e \<C>' r # \<C>) = (\<C>' \<noteq> [] \<and> r = Return\<^sub>e \<and> complete_lams \<C>' \<and> complete_lams \<C>)"
+  "complete_lams [] = False"
+| "complete_lams (PushLam\<^sub>e \<C>' # \<C>) = (\<C>' \<noteq> [Return\<^sub>e] \<and> complete_lams \<C>' \<and> complete_lams \<C>)"
+| "complete_lams (Return\<^sub>e # \<C>) = (\<C> = [])"
+| "complete_lams (Jump\<^sub>e # \<C>) = False"
 | "complete_lams (op # \<C>) = complete_lams \<C>"
 
 primrec complete_lams_val :: "closure\<^sub>e \<Rightarrow> bool" where
   "complete_lams_val (Const\<^sub>e n) = True"
-| "complete_lams_val (Lam\<^sub>e \<Delta> \<C> r) = 
-    (\<C> \<noteq> [] \<and> r = Return\<^sub>e \<and> list_all complete_lams_val \<Delta> \<and> complete_lams \<C>)"
+| "complete_lams_val (Lam\<^sub>e \<Delta> \<C>) = (\<C> \<noteq> [Return\<^sub>e] \<and> list_all complete_lams_val \<Delta> \<and> complete_lams \<C>)"
 
 fun complete_lams_frame :: "frame\<^sub>e \<Rightarrow> bool" where
-  "complete_lams_frame (\<Delta>, \<C>, r) = (list_all complete_lams_val \<Delta> \<and> complete_lams \<C> \<and> r = Return\<^sub>e)"
+  "complete_lams_frame (\<Delta>, \<C>) = (list_all complete_lams_val \<Delta> \<and> complete_lams \<C>)"
 
 primrec complete_lams_state :: "state\<^sub>e \<Rightarrow> bool" where
   "complete_lams_state (S\<^sub>e \<V> s) = (list_all complete_lams_val \<V> \<and> list_all complete_lams_frame s)"
 
+lemma complete_lams_apply [simp]: "complete_lams (e @ [Apply\<^sub>e, Return\<^sub>e]) = 
+    complete_lams (e @ [Return\<^sub>e])"
+  by (induction e rule: complete_lams.induct) simp_all
+
+lemma complete_lams_append [simp]: "complete_lams (e\<^sub>1 @ [Return\<^sub>e]) \<Longrightarrow> 
+    complete_lams (e\<^sub>2 @ [Return\<^sub>e]) \<Longrightarrow> complete_lams (e\<^sub>1 @ e\<^sub>2 @ [Apply\<^sub>e, Return\<^sub>e])"
+  by (induction e\<^sub>1 rule: complete_lams.induct) simp_all
+
+lemma encode_complete_lams [simp]: "complete_lams (encode e)"
+  by (induction e) (auto simp add: encode_def)
+
 lemma eval_complete_lams [simp]: "\<Sigma> \<leadsto>\<^sub>e \<Sigma>' \<Longrightarrow> complete_lams_state \<Sigma> \<Longrightarrow> complete_lams_state \<Sigma>'"
-  by (induction \<Sigma> \<Sigma>' rule: eval\<^sub>e.induct) auto
+  by (induction \<Sigma> \<Sigma>' rule: eval\<^sub>e.induct) (auto split: if_splits)
+
+lemma tco_not_to_jump [simp]: "\<C> \<noteq> [Return\<^sub>e] \<Longrightarrow> complete_lams \<C> \<Longrightarrow> 
+    tco_code (Apply\<^sub>e # \<C>) = Apply\<^sub>e # tco_code \<C>"
+  by (induction \<C> rule: tco_code.induct) simp_all
 
 text \<open>The \<open>iter (\<leadsto>\<^sub>e)\<close> in correctness is unusual, in that it doesn't merely mean one-or-more 
 evaluation steps, or zero-or-one, but either: clearing a dead stack frame incorporates an extra step 
@@ -107,105 +136,90 @@ for us and it takes no steps. It may seem odd that the optimized code requires t
 original code needed one, but what is actually happening is the "missing" steps from the 
 \<open>ev\<^sub>e_return\<close> are being moved there; we are still reducing the number of steps steps in total.\<close>
 
-lemma tco_to_dead_frame [simp]: "dead_frame (\<Delta>, tco_code \<C>, tco_return \<C> r) = (\<C> = [] \<and> r = Return\<^sub>e)"
-proof (induction \<C> rule: tco_code.induct)
-  case 1
-  thus ?case by (induction r) simp_all
-qed simp_all
-
-lemma tco_to_dead_frame_apply [simp]: "
-  dead_frame (map tco_val \<Delta>, tco_code (Apply\<^sub>e # \<C>), tco_return \<C> r) = (\<C> = [] \<and> r = Return\<^sub>e)"
-proof (induction \<C> rule: tco_code.induct)
-  case 1
-  thus ?case by (induction r) simp_all
-qed simp_all
-
 theorem correctness\<^sub>t\<^sub>c\<^sub>o: "\<Sigma> \<leadsto>\<^sub>e \<Sigma>' \<Longrightarrow> complete_lams_state \<Sigma> \<Longrightarrow> 
   iter (\<leadsto>\<^sub>e) (tco_state \<Sigma>) (tco_state \<Sigma>')"
 proof (induction \<Sigma> \<Sigma>' rule: eval\<^sub>e.induct)
-  case (ev\<^sub>e_lookup \<Delta> x v \<V> \<C> r s)
+  case (ev\<^sub>e_lookup \<Delta> x v \<V> \<C> s)
   thus ?case
-  proof (cases "\<C> = []")
+  proof (cases "\<C> = [Return\<^sub>e]")
     case True
     with ev\<^sub>e_lookup have  "
-      S\<^sub>e (tco_val v # map tco_val \<V>) ((map tco_val \<Delta>, tco_code \<C>, tco_return \<C> r) # tco_stack s) \<leadsto>\<^sub>e
+      S\<^sub>e (tco_val v # map tco_val \<V>) ((map tco_val \<Delta>, tco_code \<C>) # tco_stack s) \<leadsto>\<^sub>e
         S\<^sub>e (tco_val v # map tco_val \<V>) (tco_stack s)" by simp
     moreover from ev\<^sub>e_lookup have "
-      S\<^sub>e (map tco_val \<V>) ((map tco_val \<Delta>, Lookup\<^sub>e x # tco_code \<C>, tco_return \<C> r) # tco_stack s) \<leadsto>\<^sub>e
-        S\<^sub>e (tco_val v # map tco_val \<V>) ((map tco_val \<Delta>, tco_code \<C>, tco_return \<C> r) # tco_stack s)"
+      S\<^sub>e (map tco_val \<V>) ((map tco_val \<Delta>, Lookup\<^sub>e x # tco_code \<C>) # tco_stack s) \<leadsto>\<^sub>e
+        S\<^sub>e (tco_val v # map tco_val \<V>) ((map tco_val \<Delta>, tco_code \<C>) # tco_stack s)"
       by simp
-    ultimately have "iter (\<leadsto>\<^sub>e) (S\<^sub>e (map tco_val \<V>) 
-      ((map tco_val \<Delta>, Lookup\<^sub>e x # tco_code \<C>, tco_return \<C> r) # tco_stack s))
-        (S\<^sub>e (tco_val v # map tco_val \<V>) (tco_stack s))"
+    ultimately have "iter (\<leadsto>\<^sub>e) (S\<^sub>e (map tco_val \<V>) ((map tco_val \<Delta>, Lookup\<^sub>e x # tco_code \<C>) # 
+      tco_stack s)) (S\<^sub>e (tco_val v # map tco_val \<V>) (tco_stack s))"
       by (metis (no_types, lifting) iter_refl iter_step)
     with ev\<^sub>e_lookup True show ?thesis by simp
   next
     case False
-    with ev\<^sub>e_lookup have "tco_state (S\<^sub>e \<V> ((\<Delta>, Lookup\<^sub>e x # \<C>, r) # s)) \<leadsto>\<^sub>e
-      tco_state (S\<^sub>e (v # \<V>) ((\<Delta>, \<C>, r) # s))" by auto
+    with ev\<^sub>e_lookup have "tco_state (S\<^sub>e \<V> ((\<Delta>, Lookup\<^sub>e x # \<C>) # s)) \<leadsto>\<^sub>e
+      tco_state (S\<^sub>e (v # \<V>) ((\<Delta>, \<C>) # s))" by auto
     thus ?thesis by (metis iter_one)
   qed
 next
-  case (ev\<^sub>e_pushcon \<V> \<Delta> n \<C> r s)
+  case (ev\<^sub>e_pushcon \<V> \<Delta> n \<C> s)
   thus ?case
-  proof (cases "\<C> = []")
+  proof (cases "\<C> = [Return\<^sub>e]")
     case True
     with ev\<^sub>e_pushcon have "
-      S\<^sub>e (Const\<^sub>e n # map tco_val \<V>) ((map tco_val \<Delta>, tco_code \<C>, tco_return \<C> r) # tco_stack s) \<leadsto>\<^sub>e 
+      S\<^sub>e (Const\<^sub>e n # map tco_val \<V>) ((map tco_val \<Delta>, tco_code \<C>) # tco_stack s) \<leadsto>\<^sub>e 
         S\<^sub>e (Const\<^sub>e n # map tco_val \<V>) (tco_stack s)" by simp
     moreover have "
-      S\<^sub>e (map tco_val \<V>) ((map tco_val \<Delta>, PushCon\<^sub>e n # tco_code \<C>, tco_return \<C> r) # tco_stack s) \<leadsto>\<^sub>e 
-        S\<^sub>e (Const\<^sub>e n # map tco_val \<V>) ((map tco_val \<Delta>, tco_code \<C>, tco_return \<C> r) # tco_stack s)"
+      S\<^sub>e (map tco_val \<V>) ((map tco_val \<Delta>, PushCon\<^sub>e n # tco_code \<C>) # tco_stack s) \<leadsto>\<^sub>e 
+        S\<^sub>e (Const\<^sub>e n # map tco_val \<V>) ((map tco_val \<Delta>, tco_code \<C>) # tco_stack s)"
       by simp
     ultimately have "iter (\<leadsto>\<^sub>e) (S\<^sub>e (map tco_val \<V>) 
-      ((map tco_val \<Delta>, PushCon\<^sub>e n # tco_code \<C>, tco_return \<C> r) # tco_stack s))
+      ((map tco_val \<Delta>, PushCon\<^sub>e n # tco_code \<C>) # tco_stack s))
         (S\<^sub>e (Const\<^sub>e n # map tco_val \<V>) (tco_stack s))"
       by (metis (no_types, lifting) iter_refl iter_step)
     with ev\<^sub>e_pushcon True show ?thesis by simp
   next
     case False
-    hence "tco_state (S\<^sub>e \<V> ((\<Delta>, PushCon\<^sub>e n # \<C>, r) # s)) \<leadsto>\<^sub>e 
-      tco_state (S\<^sub>e (Const\<^sub>e n # \<V>) ((\<Delta>, \<C>, r) # s))" by auto
+    hence "tco_state (S\<^sub>e \<V> ((\<Delta>, PushCon\<^sub>e n # \<C>) # s)) \<leadsto>\<^sub>e tco_state (S\<^sub>e (Const\<^sub>e n # \<V>) ((\<Delta>, \<C>) # s))"
+      by auto
     thus ?thesis by (metis iter_one)
   qed
 next
-  case (ev\<^sub>e_pushlam \<V> \<Delta> \<C>' r' \<C> r s)
+  case (ev\<^sub>e_pushlam \<V> \<Delta> \<C>' \<C> s)
   thus ?case
-  proof (cases "\<C> = []")
+  proof (cases "\<C> = [Return\<^sub>e]")
     case True
-    with ev\<^sub>e_pushlam have "S\<^sub>e (Lam\<^sub>e (map tco_val \<Delta>) (tco_code \<C>') (tco_return \<C>' r') # map tco_val \<V>) 
-      ((map tco_val \<Delta>, tco_code \<C>, tco_return \<C> r) # tco_stack s) \<leadsto>\<^sub>e 
-      S\<^sub>e (Lam\<^sub>e (map tco_val \<Delta>) (tco_code \<C>') (tco_return \<C>' r') # map tco_val \<V>) (tco_stack s)" 
+    with ev\<^sub>e_pushlam have "S\<^sub>e (Lam\<^sub>e (map tco_val \<Delta>) (tco_code \<C>') # map tco_val \<V>) 
+      ((map tco_val \<Delta>, tco_code \<C>) # tco_stack s) \<leadsto>\<^sub>e 
+      S\<^sub>e (Lam\<^sub>e (map tco_val \<Delta>) (tco_code \<C>') # map tco_val \<V>) (tco_stack s)" 
         by simp
-    moreover have "S\<^sub>e (map tco_val \<V>) ((map tco_val \<Delta>, PushLam\<^sub>e (tco_code \<C>') (tco_return \<C>' r') # 
-      tco_code \<C>, tco_return \<C> r) # tco_stack s) \<leadsto>\<^sub>e 
-      S\<^sub>e (Lam\<^sub>e (map tco_val \<Delta>) (tco_code \<C>') (tco_return \<C>' r') # map tco_val \<V>) 
-      ((map tco_val \<Delta>, tco_code \<C>, tco_return \<C> r) # tco_stack s)"
+    moreover have "S\<^sub>e (map tco_val \<V>) ((map tco_val \<Delta>, PushLam\<^sub>e (tco_code \<C>') # 
+      tco_code \<C>) # tco_stack s) \<leadsto>\<^sub>e 
+      S\<^sub>e (Lam\<^sub>e (map tco_val \<Delta>) (tco_code \<C>') # map tco_val \<V>) 
+      ((map tco_val \<Delta>, tco_code \<C>) # tco_stack s)"
         by simp
-    ultimately have "iter (\<leadsto>\<^sub>e) (S\<^sub>e (map tco_val \<V>) ((map tco_val \<Delta>, PushLam\<^sub>e (tco_code \<C>') 
-      (tco_return \<C>' r') # tco_code \<C>, tco_return \<C> r) # tco_stack s))
-      (S\<^sub>e (Lam\<^sub>e (map tco_val \<Delta>) (tco_code \<C>') (tco_return \<C>' r') # map tco_val \<V>) (tco_stack s))"
+      ultimately have "iter (\<leadsto>\<^sub>e) (S\<^sub>e (map tco_val \<V>) ((map tco_val \<Delta>, PushLam\<^sub>e (tco_code \<C>') # 
+      tco_code \<C>) # tco_stack s))
+      (S\<^sub>e (Lam\<^sub>e (map tco_val \<Delta>) (tco_code \<C>') # map tco_val \<V>) (tco_stack s))"
       by (metis (no_types, lifting) iter_refl iter_step)
     with ev\<^sub>e_pushlam True show ?thesis by simp
   next
     case False
-    hence "tco_state (S\<^sub>e \<V> ((\<Delta>, PushLam\<^sub>e \<C>' r' # \<C>, r) # s)) \<leadsto>\<^sub>e 
-      tco_state (S\<^sub>e (Lam\<^sub>e \<Delta> \<C>' r' # \<V>) ((\<Delta>, \<C>, r) # s))" by simp
+    hence "tco_state (S\<^sub>e \<V> ((\<Delta>, PushLam\<^sub>e \<C>' # \<C>) # s)) \<leadsto>\<^sub>e 
+      tco_state (S\<^sub>e (Lam\<^sub>e \<Delta> \<C>' # \<V>) ((\<Delta>, \<C>) # s))" by simp
     thus ?thesis by (metis iter_one)
   qed
 next
-  case (ev\<^sub>e_apply v \<Delta>' \<C>' r' \<V> \<Delta> \<C> r s)
+  case (ev\<^sub>e_apply v \<Delta>' \<C>' \<V> \<Delta> \<C> s)
   thus ?case
-  proof (cases "\<C> = []")
+  proof (cases "\<C> = [Return\<^sub>e]")
     case True
-    with ev\<^sub>e_apply have "tco_state (S\<^sub>e (v # Lam\<^sub>e \<Delta>' \<C>' r' # \<V>) ((\<Delta>, Apply\<^sub>e # \<C>, r) # s)) \<leadsto>\<^sub>e
-      tco_state (S\<^sub>e \<V> ((v # \<Delta>', \<C>', r') # (\<Delta>, \<C>, r) # s))" by auto
+    with ev\<^sub>e_apply have "tco_state (S\<^sub>e (v # Lam\<^sub>e \<Delta>' \<C>' # \<V>) ((\<Delta>, Apply\<^sub>e # \<C>) # s)) \<leadsto>\<^sub>e
+      tco_state (S\<^sub>e \<V> ((v # \<Delta>', \<C>') # (\<Delta>, \<C>) # s))" by simp
     thus ?thesis by (metis iter_one)
   next
     case False
-    with ev\<^sub>e_apply have "tco_state (S\<^sub>e (v # Lam\<^sub>e \<Delta>' \<C>' r' # \<V>) ((\<Delta>, Apply\<^sub>e # \<C>, r) # s)) \<leadsto>\<^sub>e 
-      tco_state (S\<^sub>e \<V> ((v # \<Delta>', \<C>', r') # (\<Delta>, \<C>, r) # s))" 
-      by (cases \<C> rule: tco_code.cases) simp_all
+    with ev\<^sub>e_apply have "tco_state (S\<^sub>e (v # Lam\<^sub>e \<Delta>' \<C>' # \<V>) ((\<Delta>, Apply\<^sub>e # \<C>) # s)) \<leadsto>\<^sub>e 
+      tco_state (S\<^sub>e \<V> ((v # \<Delta>', \<C>') # (\<Delta>, \<C>) # s))" by simp
     thus ?thesis by (metis iter_one)
   qed
 qed simp_all
@@ -219,205 +233,16 @@ proof (induction \<Sigma> \<Sigma>' rule: iter.induct)
   ultimately show ?case by (metis iter_append)
 qed simp_all
 
-text \<open>We now prove the reconstruction lemmas for completeness:\<close>
-
-lemma [dest]: "(\<Delta>\<^sub>t\<^sub>c\<^sub>o, \<C>\<^sub>t\<^sub>c\<^sub>o, r\<^sub>t\<^sub>c\<^sub>o) = tco_frame f\<^sub>e \<Longrightarrow> \<exists>\<Delta>\<^sub>e \<C>\<^sub>e r\<^sub>e. f\<^sub>e = (\<Delta>\<^sub>e, \<C>\<^sub>e, r\<^sub>e) \<and> 
-    \<Delta>\<^sub>t\<^sub>c\<^sub>o = map tco_val \<Delta>\<^sub>e \<and> \<C>\<^sub>t\<^sub>c\<^sub>o = tco_code \<C>\<^sub>e \<and> r\<^sub>t\<^sub>c\<^sub>o = tco_return \<C>\<^sub>e r\<^sub>e"
-  by (induction f\<^sub>e) simp_all
-
-lemma [dest]: "f\<^sub>t\<^sub>c\<^sub>o # s\<^sub>t\<^sub>c\<^sub>o = tco_stack s\<^sub>e \<Longrightarrow> \<exists>s\<^sub>e\<^sub>1 s\<^sub>e\<^sub>2 f\<^sub>e. s\<^sub>e = s\<^sub>e\<^sub>1 @ f\<^sub>e # s\<^sub>e\<^sub>2 \<and> 
-  list_all dead_frame (map tco_frame s\<^sub>e\<^sub>1) \<and> f\<^sub>t\<^sub>c\<^sub>o = tco_frame f\<^sub>e \<and> s\<^sub>t\<^sub>c\<^sub>o = tco_stack s\<^sub>e\<^sub>2"
-proof (induction s\<^sub>e)
-  case (Cons f\<^sub>e s\<^sub>e)
-  thus ?case
-  proof (cases "dead_frame (tco_frame f\<^sub>e)")
-    case True
-    with Cons obtain s\<^sub>e\<^sub>1 s\<^sub>e\<^sub>2 f\<^sub>e' where "s\<^sub>e = s\<^sub>e\<^sub>1 @ f\<^sub>e' # s\<^sub>e\<^sub>2 \<and> list_all dead_frame (map tco_frame s\<^sub>e\<^sub>1) \<and> 
-      f\<^sub>t\<^sub>c\<^sub>o = tco_frame f\<^sub>e' \<and> s\<^sub>t\<^sub>c\<^sub>o = tco_stack s\<^sub>e\<^sub>2" by auto
-    with True have "f\<^sub>e # s\<^sub>e = (f\<^sub>e # s\<^sub>e\<^sub>1) @ f\<^sub>e' # s\<^sub>e\<^sub>2 \<and> list_all dead_frame (map tco_frame (f\<^sub>e # s\<^sub>e\<^sub>1)) \<and> 
-      f\<^sub>t\<^sub>c\<^sub>o = tco_frame f\<^sub>e' \<and> s\<^sub>t\<^sub>c\<^sub>o = tco_stack s\<^sub>e\<^sub>2" by simp
-    thus ?thesis by blast
-  next
-    case False
-    with Cons have "f\<^sub>e # s\<^sub>e = [] @ f\<^sub>e # s\<^sub>e \<and> list_all dead_frame (map tco_frame []) \<and> 
-      f\<^sub>t\<^sub>c\<^sub>o = tco_frame f\<^sub>e \<and> s\<^sub>t\<^sub>c\<^sub>o = tco_stack s\<^sub>e" by simp
-    thus ?thesis by blast
-  qed
-qed simp_all
-
-lemma [dest]: "S\<^sub>e \<V>\<^sub>t\<^sub>c\<^sub>o s\<^sub>t\<^sub>c\<^sub>o = tco_state \<Sigma>\<^sub>e \<Longrightarrow> 
-    \<exists>\<V>\<^sub>e s\<^sub>e. \<Sigma>\<^sub>e = S\<^sub>e \<V>\<^sub>e s\<^sub>e \<and> \<V>\<^sub>t\<^sub>c\<^sub>o = map tco_val \<V>\<^sub>e \<and> s\<^sub>t\<^sub>c\<^sub>o = tco_stack s\<^sub>e"
-  by (induction \<Sigma>\<^sub>e) simp_all
-
-text \<open>Completeness then follows:\<close>
-
-theorem complete\<^sub>t\<^sub>c\<^sub>o [simp]: "tco_state \<Sigma>\<^sub>e \<leadsto>\<^sub>e \<Sigma>\<^sub>t\<^sub>c\<^sub>o' \<Longrightarrow> 
-  \<exists>\<Sigma>\<^sub>e'. iter (\<leadsto>\<^sub>e) \<Sigma>\<^sub>e \<Sigma>\<^sub>e' \<and> \<Sigma>\<^sub>t\<^sub>c\<^sub>o' = tco_state \<Sigma>\<^sub>e'"
-proof (induction "tco_state \<Sigma>\<^sub>e" \<Sigma>\<^sub>t\<^sub>c\<^sub>o' rule: eval\<^sub>e.induct)
-  case (ev\<^sub>e_lookup \<Delta>\<^sub>t\<^sub>c\<^sub>o x v \<V>\<^sub>t\<^sub>c\<^sub>o \<C>\<^sub>t\<^sub>c\<^sub>o r\<^sub>t\<^sub>c\<^sub>o s\<^sub>t\<^sub>c\<^sub>o)
-  then obtain \<V>\<^sub>e s\<^sub>e\<^sub>1 s\<^sub>e\<^sub>2 \<Delta>\<^sub>e \<C>\<^sub>e r\<^sub>e where "\<Sigma>\<^sub>e = S\<^sub>e \<V>\<^sub>e (s\<^sub>e\<^sub>1 @ (\<Delta>\<^sub>e, \<C>\<^sub>e, r\<^sub>e) # s\<^sub>e\<^sub>2) \<and> \<V>\<^sub>t\<^sub>c\<^sub>o = map tco_val \<V>\<^sub>e \<and> 
-    list_all dead_frame (map tco_frame s\<^sub>e\<^sub>1) \<and> \<Delta>\<^sub>t\<^sub>c\<^sub>o = map tco_val \<Delta>\<^sub>e \<and> Lookup\<^sub>e x # \<C>\<^sub>t\<^sub>c\<^sub>o = tco_code \<C>\<^sub>e \<and> 
-      r\<^sub>t\<^sub>c\<^sub>o = tco_return \<C>\<^sub>e r\<^sub>e \<and> s\<^sub>t\<^sub>c\<^sub>o = tco_stack s\<^sub>e\<^sub>2" by fast
-
-
-
-  have "iter (\<leadsto>\<^sub>e) \<Sigma>\<^sub>e \<Sigma>\<^sub>e' \<and> S\<^sub>e (v # \<V>\<^sub>t\<^sub>c\<^sub>o) ((\<Delta>\<^sub>t\<^sub>c\<^sub>o, \<C>\<^sub>t\<^sub>c\<^sub>o, r\<^sub>t\<^sub>c\<^sub>o) # s\<^sub>t\<^sub>c\<^sub>o) = tco_state \<Sigma>\<^sub>e'" by simp
-  thus ?case by blast
-next
-  case (ev\<^sub>e_pushcon \<V>\<^sub>t\<^sub>c\<^sub>o \<Delta>\<^sub>t\<^sub>c\<^sub>o n \<C>\<^sub>t\<^sub>c\<^sub>o r\<^sub>t\<^sub>c\<^sub>o s\<^sub>t\<^sub>c\<^sub>o)
-  then obtain \<V>\<^sub>e s\<^sub>e\<^sub>1 s\<^sub>e\<^sub>2 f\<^sub>e where "\<Sigma>\<^sub>e = S\<^sub>e \<V>\<^sub>e (s\<^sub>e\<^sub>1 @ f\<^sub>e # s\<^sub>e\<^sub>2) \<and> \<V>\<^sub>t\<^sub>c\<^sub>o = map tco_val \<V>\<^sub>e \<and> 
-    list_all dead_frame (map tco_frame s\<^sub>e\<^sub>1) \<and> (\<Delta>\<^sub>t\<^sub>c\<^sub>o, PushCon\<^sub>e n # \<C>\<^sub>t\<^sub>c\<^sub>o, r\<^sub>t\<^sub>c\<^sub>o) = tco_frame f\<^sub>e \<and> 
-      s\<^sub>t\<^sub>c\<^sub>o = tco_stack s\<^sub>e\<^sub>2" by blast
-
-  then show ?case by simp
-next
-  case (ev\<^sub>e_pushlam \<V>\<^sub>t\<^sub>c\<^sub>o \<Delta>\<^sub>t\<^sub>c\<^sub>o \<C>' r' \<C>\<^sub>t\<^sub>c\<^sub>o r\<^sub>t\<^sub>c\<^sub>o s\<^sub>t\<^sub>c\<^sub>o)
-  then obtain \<V>\<^sub>e s\<^sub>e\<^sub>1 s\<^sub>e\<^sub>2 f\<^sub>e where "\<Sigma>\<^sub>e = S\<^sub>e \<V>\<^sub>e (s\<^sub>e\<^sub>1 @ f\<^sub>e # s\<^sub>e\<^sub>2) \<and> \<V>\<^sub>t\<^sub>c\<^sub>o = map tco_val \<V>\<^sub>e \<and> 
-    list_all dead_frame (map tco_frame s\<^sub>e\<^sub>1) \<and> (\<Delta>\<^sub>t\<^sub>c\<^sub>o, PushLam\<^sub>e \<C>' r' # \<C>\<^sub>t\<^sub>c\<^sub>o, r\<^sub>t\<^sub>c\<^sub>o) = tco_frame f\<^sub>e \<and> 
-      s\<^sub>t\<^sub>c\<^sub>o = tco_stack s\<^sub>e\<^sub>2" by blast
-
-  then show ?case by simp
-next
-  case (ev\<^sub>e_apply v \<Delta>' \<C>' r' \<V>\<^sub>t\<^sub>c\<^sub>o \<Delta>\<^sub>t\<^sub>c\<^sub>o \<C>\<^sub>t\<^sub>c\<^sub>o r\<^sub>t\<^sub>c\<^sub>o s\<^sub>t\<^sub>c\<^sub>o)
-  then obtain \<V>\<^sub>e s\<^sub>e\<^sub>1 s\<^sub>e\<^sub>2 f\<^sub>e where "\<Sigma>\<^sub>e = S\<^sub>e \<V>\<^sub>e (s\<^sub>e\<^sub>1 @ f\<^sub>e # s\<^sub>e\<^sub>2) \<and> (v # Lam\<^sub>e \<Delta>' \<C>' r' # \<V>\<^sub>t\<^sub>c\<^sub>o) = map tco_val \<V>\<^sub>e \<and> 
-    list_all dead_frame (map tco_frame s\<^sub>e\<^sub>1) \<and> (\<Delta>\<^sub>t\<^sub>c\<^sub>o, Apply\<^sub>e # \<C>\<^sub>t\<^sub>c\<^sub>o, r\<^sub>t\<^sub>c\<^sub>o) = tco_frame f\<^sub>e \<and> 
-      s\<^sub>t\<^sub>c\<^sub>o = tco_stack s\<^sub>e\<^sub>2" by blast
-
-  then show ?case by simp
-next
-  case (ev\<^sub>e_return \<V>\<^sub>t\<^sub>c\<^sub>o \<Delta>\<^sub>t\<^sub>c\<^sub>o s\<^sub>t\<^sub>c\<^sub>o)
-  then obtain \<V>\<^sub>e s\<^sub>e\<^sub>1 s\<^sub>e\<^sub>2 f\<^sub>e where "\<Sigma>\<^sub>e = S\<^sub>e \<V>\<^sub>e (s\<^sub>e\<^sub>1 @ f\<^sub>e # s\<^sub>e\<^sub>2) \<and> \<V>\<^sub>t\<^sub>c\<^sub>o = map tco_val \<V>\<^sub>e \<and> 
-    list_all dead_frame (map tco_frame s\<^sub>e\<^sub>1) \<and> (\<Delta>\<^sub>t\<^sub>c\<^sub>o, [], Return\<^sub>e) = tco_frame f\<^sub>e \<and> 
-      s\<^sub>t\<^sub>c\<^sub>o = tco_stack s\<^sub>e\<^sub>2" by blast
-
-  then show ?case by simp
-next
-  case (ev\<^sub>e_jump v \<Delta>' \<C>' r' \<V>\<^sub>t\<^sub>c\<^sub>o \<Delta>\<^sub>t\<^sub>c\<^sub>o s\<^sub>t\<^sub>c\<^sub>o)
-  then obtain \<V>\<^sub>e s\<^sub>e\<^sub>1 s\<^sub>e\<^sub>2 f\<^sub>e where "\<Sigma>\<^sub>e = S\<^sub>e \<V>\<^sub>e (s\<^sub>e\<^sub>1 @ f\<^sub>e # s\<^sub>e\<^sub>2) \<and> (v # Lam\<^sub>e \<Delta>' \<C>' r' # \<V>\<^sub>t\<^sub>c\<^sub>o) = map tco_val \<V>\<^sub>e \<and> 
-    list_all dead_frame (map tco_frame s\<^sub>e\<^sub>1) \<and> (\<Delta>\<^sub>t\<^sub>c\<^sub>o, [], Jump\<^sub>e) = tco_frame f\<^sub>e \<and> 
-      s\<^sub>t\<^sub>c\<^sub>o = tco_stack s\<^sub>e\<^sub>2" by blast
-
-  then show ?case by simp
-qed
-
-(*
-lemma [simp]: "cd \<noteq> [] \<Longrightarrow> tco_r (op # cd) = tco_r cd"
-  by (induction op) (simp_all split: list.splits)
-
-lemma tco_r_append [simp]: "cd' \<noteq> [] \<Longrightarrow> tco_r (cd @ cd') = tco_r cd'"
-  by (induction cd) simp_all
-
-lemma [simp]: "cd \<noteq> [] \<Longrightarrow> cd' \<noteq> [] \<Longrightarrow> tco_cd (cd @ cd') \<noteq> []"
-  by (induction cd rule: tco_cd.induct) (simp_all split: list.splits)
-
-lemma [dest]: "(env, cd, r) # sfs = tco_stack sfs' \<Longrightarrow> \<exists>dsfs env' cd' sfs''. 
-  sfs' = dsfs @ (env', cd') # sfs'' \<and> env = map tco_val env' \<and> cd = tco_cd cd' \<and> 
-    r = tco_r cd' \<and> list_all dead_frame dsfs \<and> sfs = tco_stack sfs''"
-proof (induction sfs')
-  case (Cons sf sfs')
-  thus ?case
-  proof (induction sf)
-    case (Pair env' cd')
-    thus ?case
-    proof (induction cd' rule: tco_cd.induct)
-      case 1
-      then obtain dsfs env'' cd' sfs'' where X: "sfs' = dsfs @ (env'', cd') # sfs'' \<and> 
-        env = map tco_val env'' \<and> cd = tco_cd cd' \<and> r = tco_r cd' \<and> list_all dead_frame dsfs \<and> 
-          sfs = tco_stack sfs''" by auto
-      hence "\<exists>dsfsx. (env', []) # dsfs @ (env'', cd') # sfs'' = dsfsx @ (env'', cd') # sfs'' \<and> 
-          list_all dead_frame dsfsx \<and> sfs = tco_stack sfs''" by simp
-      hence "\<exists>dsfsx sfs'''. 
-        (env', []) # dsfs @ (env'', cd') # sfs'' = dsfsx @ (env'', cd') # sfs''' \<and> 
-          list_all dead_frame dsfsx \<and> sfs = tco_stack sfs'''" by fastforce
-      with X show ?case by fastforce
-    next
-      case (2 x cd')
-      hence "env = map tco_val env' \<and> cd = Lookup\<^sub>e x # tco_cd cd' \<and> r = tco_r cd' \<and> 
-        sfs = tco_stack sfs'" by simp
-      thus ?case by fastforce
-    next
-      case (3 k cd')
-      hence "env = map tco_val env' \<and> cd = PushCon\<^sub>e k # tco_cd cd' \<and> r = tco_r cd' \<and> 
-        sfs = tco_stack sfs'" by simp
-      thus ?case by fastforce
-    next
-      case (4 cd\<^sub>e cd')
-      hence "env = map tco_val env' \<and> cd = PushLam\<^sub>e (tco_cd cd\<^sub>e) (tco_r cd\<^sub>e) # tco_cd cd' \<and> 
-        r = tco_r cd' \<and> sfs = tco_stack sfs'" by simp
-      thus ?case by fastforce
-    next
-      case (5 cd')
-      thus ?case
-      proof (cases cd')
-        case Nil
-        moreover with 5 have "env = map tco_val env' \<and> cd = [] \<and> r = Jump\<^sub>e \<and> sfs = tco_stack sfs'" 
-          by simp
-        ultimately show ?thesis by fastforce
-      next
-        case (Cons op cd'')
-        moreover with 5 have "env = map tco_val env' \<and> cd = Apply\<^sub>e # tco_cd (op # cd'') \<and> 
-          r = tco_r (op # cd'') \<and> sfs = tco_stack sfs'" by simp
-        ultimately show ?thesis by fastforce
-      qed
-    qed
-  qed
-qed simp_all
-
-lemma [dest]: "S\<^sub>e vs ((env, cd, r) # sfs) = tco_state \<Sigma> \<Longrightarrow> \<exists>dsfs vs' env' cd' sfs'. 
-  \<Sigma> = S\<^sub>e vs' (dsfs @ (env', cd') # sfs') \<and> vs = map tco_val vs' \<and> env = map tco_val env' \<and> 
-    cd = tco_cd cd' \<and> r = tco_r cd' \<and> list_all dead_frame dsfs \<and> sfs = tco_stack sfs'"
-  by (induction \<Sigma>) auto
-
-lemma [dest]: "Lookup\<^sub>e x # cd = tco_cd cd' \<Longrightarrow> \<exists>cd''. cd' = Lookup\<^sub>e x # cd'' \<and> cd = tco_cd cd''"
-  by (induction cd' rule: tco_cd.induct) (simp_all split: list.splits)
-
-lemma [dest]: "PushCon\<^sub>e k # cd = tco_cd cd' \<Longrightarrow> \<exists>cd''. cd' = PushCon\<^sub>e k # cd'' \<and> cd = tco_cd cd''"
-  by (induction cd' rule: tco_cd.induct) (simp_all split: list.splits)
-
-lemma [dest]: "PushLam\<^sub>e cd' r # cd = tco_cd cd\<^sub>t \<Longrightarrow> \<exists>cd\<^sub>t' cd\<^sub>t''. cd\<^sub>t = PushLam\<^sub>e cd\<^sub>t'' # cd\<^sub>t' \<and> 
-    cd = tco_cd cd\<^sub>t' \<and> r = tco_r cd\<^sub>t'' \<and> cd' = tco_cd cd\<^sub>t''"
-  by (induction cd\<^sub>t rule: tco_cd.induct) (simp_all split: list.splits)
-
-lemma [dest]: "Apply\<^sub>e # cd = tco_cd cd' \<Longrightarrow> 
-    \<exists>op cd''. cd' = Apply\<^sub>e # op # cd'' \<and> cd = tco_cd (op # cd'')"
-  by (induction cd' rule: tco_cd.induct) (simp_all split: list.splits)
-
-lemma [dest]: "Const\<^sub>e k = tco_val v \<Longrightarrow> v = Const\<^sub>e k"
-  by (induction v) simp_all
-
-lemma [dest]: "Lam\<^sub>e env cd r = tco_val v \<Longrightarrow> 
-    \<exists>env\<^sub>t cd\<^sub>t. v = Lam\<^sub>e env\<^sub>t cd\<^sub>t \<and> env = map tco_val env\<^sub>t \<and> cd = tco_cd cd\<^sub>t \<and> r = tco_r cd\<^sub>t"
-  by (induction v) simp_all
-
-lemma [dest]: "Return\<^sub>e = tco_r cd \<Longrightarrow> [] = tco_cd cd \<Longrightarrow> cd = []"
-  by (induction cd rule: tco_cd.induct) (simp_all split: list.splits)
-
-lemma [dest]: "Jump\<^sub>e = tco_r cd \<Longrightarrow> [] = tco_cd cd \<Longrightarrow> cd = [Apply\<^sub>e]"
-  by (induction cd rule: tco_cd.induct) (simp_all split: list.splits)
-
-lemma [simp]: "list_all dead_frame dsfs \<Longrightarrow> iter (\<leadsto>\<^sub>e) (S\<^sub>e vs (dsfs @ sfs)) (S\<^sub>e vs sfs)"
-proof (induction dsfs)
-  case (Cons sf dsfs)
-  then obtain vs' where "sf = (vs', [])" by (cases sf) simp_all
-  hence "S\<^sub>e vs ((sf # dsfs) @ sfs) \<leadsto>\<^sub>e S\<^sub>e vs (dsfs @ sfs)" by simp
-  with Cons show ?case by simp
-qed simp_all
-
-lemma [simp]: "\<not> live_frame fr \<Longrightarrow> iter (\<leadsto>\<^sub>e) (S\<^sub>e vs (fr # sfs)) (S\<^sub>e vs sfs)"
-proof (induction fr rule: live_frame.induct)
-  case (1 env)
-  hence "S\<^sub>e vs ((env, [], Return\<^sub>e) # sfs) \<leadsto>\<^sub>e S\<^sub>e vs sfs" by simp
-  thus ?case by (metis iter_one)
-qed simp_all
-
-lemma [simp]: "tco_cd (op # cd) = [] \<Longrightarrow> tco_r (op # cd) = Jump\<^sub>e"
-  by (induction op) (simp_all split: list.splits)
-
-lemma [simp]: "live_frame (env, cd, Jump\<^sub>e)"
-  by (induction cd) simp_all
-
-lemma tco_never_dead [simp]: "live_frame (env, tco_cd (op # cd), tco_r (op # cd))"
-  by (induction op) (simp_all split: list.splits)
-*)
+text \<open>Completeness would then follow, after the usual reconstruction lemmas. However, the way that 
+optimized steps don't quite align with unoptimized steps mentioned above now comes back to bite, 
+unpleasantly. Optimized evaluation may put us in a state that simply has no unoptimized equivalent; 
+we have to sometimes take an additional optimized step to get back to matching states. The actual
+statement would end up being 
+  \<open>tco_state \<Sigma>\<^sub>e \<leadsto>\<^sub>e \<Sigma>\<^sub>t\<^sub>c\<^sub>o' \<Longrightarrow> 
+    \<exists>\<Sigma>\<^sub>e'' \<Sigma>\<^sub>t\<^sub>c\<^sub>o''. iter (\<leadsto>\<^sub>e) \<Sigma>\<^sub>t\<^sub>c\<^sub>o' \<Sigma>\<^sub>t\<^sub>c\<^sub>o'' \<and> iter (\<leadsto>\<^sub>e) \<Sigma>\<^sub>e \<Sigma>\<^sub>e'' \<and> \<Sigma>\<^sub>t\<^sub>c\<^sub>o'' = tco_state \<Sigma>\<^sub>e''\<close>
+with the first iter indicating zero-or-one, and the second one-or-more. Rather than deal with this
+complication, we note that completeness is the only part of this that we need, and skip it. (We will 
+later encounter the exact same evaluation-mismatch problem, and abandon completeness with the exact
+same justification, when we move to assembly code in stage 12.)\<close>
 
 end
