06TreeCode/TreeCode.thy
@@ -14,34 +14,33 @@ text \<open>Our tree-code contains one constructor per expression constructor. T
 application is now an operation without arguments; we have restructured the expression tree into a 
 postfix form. Lambda-abstractions keep their sub-codeblock, however (hence the name "tree" code). We 
 Will eliminate this too, but not for a few stages yet. We also create an explicit return operation, 
-to pop frames off the stack, rather than simply doing so when we run out of code. This will help 
-make it clear where blocks end, once we no longer have the luxury of tree-structured code in the 
-next stage - but the second operation \<open>Jump\<^sub>e\<close>, which we do not use yet, will also come in useful for 
-tail-call optimization soon.\<close>
-
-datatype return\<^sub>e =
-  Return\<^sub>e
-  | Jump\<^sub>e
+to pop frames off the stack, rather than simply doing so when we run out of code. We arrange - 
+although we do not enforce syntactically - that every code block ends with a \<open>Return\<^sub>e\<close>. This will 
+help make it clear where blocks end, once we no longer have the luxury of tree-structured code in 
+the next stage - but the second return-like operation \<open>Jump\<^sub>e\<close>, which we do not use yet, will also 
+come in useful for tail-call optimization soon.\<close>
 
 datatype code\<^sub>e = 
   Lookup\<^sub>e nat
   | PushCon\<^sub>e nat
-  | PushLam\<^sub>e "code\<^sub>e list" return\<^sub>e
+  | PushLam\<^sub>e "code\<^sub>e list"
   | Apply\<^sub>e
+  | Return\<^sub>e
+  | Jump\<^sub>e
 
 text \<open>Our closure-values remain the same, with just a change from a function body to a function 
-codeblock and return operation in closures-proper.\<close>
+codeblock in closures-proper.\<close>
 
 datatype closure\<^sub>e = 
   Const\<^sub>e nat
-  | Lam\<^sub>e "closure\<^sub>e list" "code\<^sub>e list" return\<^sub>e
+  | Lam\<^sub>e "closure\<^sub>e list" "code\<^sub>e list"
 
 text \<open>Our state, however, is greatly changed. In particular, the call stack has to be divided in 
 two: part of it becomes the call stack proper, with frames containing the call environment and a 
 block of yet-to-be-executed code, and the remainder becomes a value stack that \<open>PushX\<^sub>e\<close> operations 
 push onto and \<open>Apply\<^sub>e\<close> operations pop off.\<close>
 
-type_synonym frame\<^sub>e = "closure\<^sub>e list \<times> code\<^sub>e list \<times> return\<^sub>e"
+type_synonym frame\<^sub>e = "closure\<^sub>e list \<times> code\<^sub>e list"
 
 datatype state\<^sub>e = S\<^sub>e "closure\<^sub>e list" "frame\<^sub>e list"
 
@@ -49,19 +48,19 @@ text \<open>Evaluation is now directed entirely by the code in the topmost calls
 \<open>PushX\<close> push onto the value stack (the former looking up its closure-value from the topmost 
 callstack frame's environment); \<open>Apply\<^sub>e\<close> pops two values (the second of which should be a \<open>Lam\<^sub>e\<close>, to 
 be applied), and pushes a new callstack frame using the closure's environment and codeblock. When 
-the code in a callstack frame is exhausted, we follow the \<open>Return\<^sub>e\<close> operation and pop that frame off 
-the callstack. (The final \<open>ev\<^sub>e_jump\<close> transition we will cover later.)\<close>
+we reach the \<open>Return\<^sub>e\<close> operation (which should always be when the code in a callstack frame is 
+exhausted), we pop that frame off the callstack. (The final \<open>ev\<^sub>e_jump\<close> transition we will cover 
+later.)\<close>
 
 inductive eval\<^sub>e :: "state\<^sub>e \<Rightarrow> state\<^sub>e \<Rightarrow> bool" (infix "\<leadsto>\<^sub>e" 50) where
   ev\<^sub>e_lookup [simp]: "lookup \<Delta> x = Some v \<Longrightarrow> 
-    S\<^sub>e \<V> ((\<Delta>, Lookup\<^sub>e x # \<C>, r) # s) \<leadsto>\<^sub>e S\<^sub>e (v # \<V>) ((\<Delta>, \<C>, r) # s)"
-| ev\<^sub>e_pushcon [simp]: "S\<^sub>e \<V> ((\<Delta>, PushCon\<^sub>e n # \<C>, r) # s) \<leadsto>\<^sub>e S\<^sub>e (Const\<^sub>e n # \<V>) ((\<Delta>, \<C>, r) # s)"
-| ev\<^sub>e_pushlam [simp]: "S\<^sub>e \<V> ((\<Delta>, PushLam\<^sub>e \<C>' r' # \<C>, r) # s) \<leadsto>\<^sub>e 
-    S\<^sub>e (Lam\<^sub>e \<Delta> \<C>' r' # \<V>) ((\<Delta>, \<C>, r) # s)"
-| ev\<^sub>e_apply [simp]: "S\<^sub>e (v # Lam\<^sub>e \<Delta>' \<C>' r' # \<V>) ((\<Delta>, Apply\<^sub>e # \<C>, r) # s) \<leadsto>\<^sub>e 
-    S\<^sub>e \<V> ((v # \<Delta>', \<C>', r') # (\<Delta>, \<C>, r) # s)"
-| ev\<^sub>e_return [simp]: "S\<^sub>e \<V> ((\<Delta>, [], Return\<^sub>e) # s) \<leadsto>\<^sub>e S\<^sub>e \<V> s"
-| ev\<^sub>e_jump [simp]: "S\<^sub>e (v # Lam\<^sub>e \<Delta>' \<C>' r' # \<V>) ((\<Delta>, [], Jump\<^sub>e) # s) \<leadsto>\<^sub>e S\<^sub>e \<V> ((v # \<Delta>', \<C>', r') # s)"
+    S\<^sub>e \<V> ((\<Delta>, Lookup\<^sub>e x # \<C>) # s) \<leadsto>\<^sub>e S\<^sub>e (v # \<V>) ((\<Delta>, \<C>) # s)"
+| ev\<^sub>e_pushcon [simp]: "S\<^sub>e \<V> ((\<Delta>, PushCon\<^sub>e n # \<C>) # s) \<leadsto>\<^sub>e S\<^sub>e (Const\<^sub>e n # \<V>) ((\<Delta>, \<C>) # s)"
+| ev\<^sub>e_pushlam [simp]: "S\<^sub>e \<V> ((\<Delta>, PushLam\<^sub>e \<C>' # \<C>) # s) \<leadsto>\<^sub>e S\<^sub>e (Lam\<^sub>e \<Delta> \<C>' # \<V>) ((\<Delta>, \<C>) # s)"
+| ev\<^sub>e_apply [simp]: "S\<^sub>e (v # Lam\<^sub>e \<Delta>' \<C>' # \<V>) ((\<Delta>, Apply\<^sub>e # \<C>) # s) \<leadsto>\<^sub>e 
+    S\<^sub>e \<V> ((v # \<Delta>', \<C>') # (\<Delta>, \<C>) # s)"
+| ev\<^sub>e_return [simp]: "S\<^sub>e \<V> ((\<Delta>, Return\<^sub>e # \<C>) # s) \<leadsto>\<^sub>e S\<^sub>e \<V> s"
+| ev\<^sub>e_jump [simp]: "S\<^sub>e (v # Lam\<^sub>e \<Delta>' \<C>' # \<V>) ((\<Delta>, Jump\<^sub>e # \<C>) # s) \<leadsto>\<^sub>e S\<^sub>e \<V> ((v # \<Delta>', \<C>') # s)"
 
 text \<open>Without typing, our list of safety properties has become quite short: just determinism. We 
 could still type our codeblocks, and thence our state; we would need to give each tree-code 
