06TreeCode/TreeCodeConversion.thy
@@ -11,17 +11,20 @@ tree-code closures-values are just encoded stack closure-values. We add a \<open
 the end of ever code block, too; we never encode the \<open>Jump\<^sub>e\<close> operation. Its place will come a little 
 later.\<close>
 
-primrec encode :: "expr\<^sub>d \<Rightarrow> code\<^sub>e list" where
-  "encode (Var\<^sub>d x) = [Lookup\<^sub>e x]"
-| "encode (Const\<^sub>d n) = [PushCon\<^sub>e n]"
-| "encode (Lam\<^sub>d t e) = [PushLam\<^sub>e (encode e) Return\<^sub>e]"
-| "encode (App\<^sub>d e\<^sub>1 e\<^sub>2) = encode e\<^sub>1 @ encode e\<^sub>2 @ [Apply\<^sub>e]"
+primrec encode' :: "expr\<^sub>d \<Rightarrow> code\<^sub>e list" where
+  "encode' (Var\<^sub>d x) = [Lookup\<^sub>e x]"
+| "encode' (Const\<^sub>d n) = [PushCon\<^sub>e n]"
+| "encode' (Lam\<^sub>d t e) = [PushLam\<^sub>e (encode' e @ [Return\<^sub>e])]"
+| "encode' (App\<^sub>d e\<^sub>1 e\<^sub>2) = encode' e\<^sub>1 @ encode' e\<^sub>2 @ [Apply\<^sub>e]"
+
+definition encode :: "expr\<^sub>d \<Rightarrow> code\<^sub>e list" where
+  "encode e \<equiv> encode' e @ [Return\<^sub>e]"
 
 primrec encode_closure :: "closure\<^sub>c \<Rightarrow> closure\<^sub>e" where
   "encode_closure (Const\<^sub>c n) = Const\<^sub>e n"
-| "encode_closure (Lam\<^sub>c t \<Delta> e) = Lam\<^sub>e (map encode_closure \<Delta>) (encode e) Return\<^sub>e"
+| "encode_closure (Lam\<^sub>c t \<Delta> e) = Lam\<^sub>e (map encode_closure \<Delta>) (encode e)"
 
-lemma tl_encode [simp]: "tl (encode e @ \<C>) = tl (encode e) @ \<C>"
+lemma tl_encode [simp]: "tl (encode' e @ \<C>) = tl (encode' e) @ \<C>"
   by (induction e arbitrary: \<C>) simp_all
 
 text \<open>It is the callstack where things get complicated: we have to divide the stack into a 
@@ -43,14 +46,14 @@ what environment) callstack frames begin.\<close>
 
 fun prepend_to_top_frame :: "code\<^sub>e list \<Rightarrow> frame\<^sub>e list \<Rightarrow> frame\<^sub>e list" where
   "prepend_to_top_frame \<C> [] = []"
-| "prepend_to_top_frame \<C> ((\<Delta>, \<C>', r) # s\<^sub>e) = (\<Delta>, \<C> @ \<C>', r) # s\<^sub>e"
+| "prepend_to_top_frame \<C> ((\<Delta>, \<C>') # s\<^sub>e) = (\<Delta>, \<C> @ \<C>') # s\<^sub>e"
 
 fun stack_from_stack :: "frame\<^sub>c list \<Rightarrow> frame\<^sub>e list" where
   "stack_from_stack [] = []"
 | "stack_from_stack (FApp1\<^sub>c \<Delta>' e # s\<^sub>c) = 
-    prepend_to_top_frame (encode e @ [Apply\<^sub>e]) (stack_from_stack s\<^sub>c)"
+    prepend_to_top_frame (encode' e @ [Apply\<^sub>e]) (stack_from_stack s\<^sub>c)"
 | "stack_from_stack (FApp2\<^sub>c c # s\<^sub>c) = prepend_to_top_frame [Apply\<^sub>e] (stack_from_stack s\<^sub>c)"
-| "stack_from_stack (FReturn\<^sub>c \<Delta> # s\<^sub>c) = (map encode_closure \<Delta>, [], Return\<^sub>e) # stack_from_stack s\<^sub>c"
+| "stack_from_stack (FReturn\<^sub>c \<Delta> # s\<^sub>c) = (map encode_closure \<Delta>, [Return\<^sub>e]) # stack_from_stack s\<^sub>c"
 
 lemma prepend_nil [simp]: "prepend_to_top_frame [] s\<^sub>e = s\<^sub>e"
   by (induction "[] :: code\<^sub>e list" s\<^sub>e rule: prepend_to_top_frame.induct) simp_all
@@ -65,7 +68,7 @@ frame.\<close>
 
 primrec encode_state :: "state\<^sub>c \<Rightarrow> state\<^sub>e" where
   "encode_state (SE\<^sub>c s\<^sub>c \<Delta> e) = 
-    S\<^sub>e (vals_from_stack s\<^sub>c) (prepend_to_top_frame (encode e) (stack_from_stack s\<^sub>c))"
+    S\<^sub>e (vals_from_stack s\<^sub>c) (prepend_to_top_frame (encode' e) (stack_from_stack s\<^sub>c))"
 | "encode_state (SC\<^sub>c s\<^sub>c c) = S\<^sub>e (encode_closure c # vals_from_stack s\<^sub>c) (stack_from_stack s\<^sub>c)"
 
 text \<open>Because the conversion functions run forwards, we can once again prove correctness easily.
@@ -74,7 +77,7 @@ We again have to use \<open>iter\<close> in our statement of the theorem, becaus
 steps (\<open>ret\<^sub>c_app1\<close> and \<open>ret\<^sub>c_app2\<close>) are not matched by any steps in the tree-code evaluation.\<close>
 
 lemma lookup_latest [dest]: "latest_environment s\<^sub>c = Some \<Delta> \<Longrightarrow> 
-    \<exists>\<C> s\<^sub>e. stack_from_stack s\<^sub>c = (map encode_closure \<Delta>, \<C>, Return\<^sub>e) # s\<^sub>e"
+    \<exists>\<C> s\<^sub>e. stack_from_stack s\<^sub>c = (map encode_closure \<Delta>, \<C>) # s\<^sub>e"
   by (induction s\<^sub>c rule: stack_from_stack.induct) auto
 
 theorem correct\<^sub>e [simp]: "\<Sigma> \<leadsto>\<^sub>c \<Sigma>' \<Longrightarrow> \<Sigma> :\<^sub>c t \<Longrightarrow> iter (\<leadsto>\<^sub>e) (encode_state \<Sigma>) (encode_state \<Sigma>')"
@@ -82,59 +85,57 @@ proof (induction \<Sigma> \<Sigma>' rule: eval\<^sub>c.induct)
   case (ev\<^sub>c_var \<Delta> x c s\<^sub>c)
   then obtain t' \<Gamma> where "(s\<^sub>c :\<^sub>c t' \<rightarrow> t) \<and> (\<Delta> :\<^sub>c\<^sub>l\<^sub>s \<Gamma>) \<and> latest_environment s\<^sub>c = Some \<Delta> \<and> 
     lookup \<Gamma> x = Some t'" by fastforce
-  then obtain \<C> s\<^sub>e where S: "stack_from_stack s\<^sub>c = (map encode_closure \<Delta>, \<C>, Return\<^sub>e) # s\<^sub>e" by auto
-  with ev\<^sub>c_var have "S\<^sub>e (vals_from_stack s\<^sub>c) ((map encode_closure \<Delta>, Lookup\<^sub>e x # \<C>, Return\<^sub>e) # s\<^sub>e) \<leadsto>\<^sub>e 
-    S\<^sub>e (encode_closure c # vals_from_stack s\<^sub>c) ((map encode_closure \<Delta>, \<C>, Return\<^sub>e) # s\<^sub>e)" by simp
-  hence "iter (\<leadsto>\<^sub>e) (S\<^sub>e (vals_from_stack s\<^sub>c) ((map encode_closure \<Delta>, Lookup\<^sub>e x # \<C>, Return\<^sub>e) # s\<^sub>e))
-    (S\<^sub>e (encode_closure c # vals_from_stack s\<^sub>c) ((map encode_closure \<Delta>, \<C>, Return\<^sub>e) # s\<^sub>e))" 
+  then obtain \<C> s\<^sub>e where S: "stack_from_stack s\<^sub>c = (map encode_closure \<Delta>, \<C>) # s\<^sub>e" by auto
+  with ev\<^sub>c_var have "S\<^sub>e (vals_from_stack s\<^sub>c) ((map encode_closure \<Delta>, Lookup\<^sub>e x # \<C>) # s\<^sub>e) \<leadsto>\<^sub>e 
+    S\<^sub>e (encode_closure c # vals_from_stack s\<^sub>c) ((map encode_closure \<Delta>, \<C>) # s\<^sub>e)" by simp
+  hence "iter (\<leadsto>\<^sub>e) (S\<^sub>e (vals_from_stack s\<^sub>c) ((map encode_closure \<Delta>, Lookup\<^sub>e x # \<C>) # s\<^sub>e))
+    (S\<^sub>e (encode_closure c # vals_from_stack s\<^sub>c) ((map encode_closure \<Delta>, \<C>) # s\<^sub>e))" 
       by (metis iter_one)
   with S show ?case by simp
 next
   case (ev\<^sub>c_con s\<^sub>c \<Delta> n)
   then obtain \<Gamma> where "(s\<^sub>c :\<^sub>c Num \<rightarrow> t) \<and> (\<Delta> :\<^sub>c\<^sub>l\<^sub>s \<Gamma>) \<and> latest_environment s\<^sub>c = Some \<Delta>" by fastforce
-  then obtain \<C> s\<^sub>e where S: "stack_from_stack s\<^sub>c = (map encode_closure \<Delta>, \<C>, Return\<^sub>e) # s\<^sub>e" by auto
-  have "S\<^sub>e (vals_from_stack s\<^sub>c) ((map encode_closure \<Delta>, PushCon\<^sub>e n # \<C>, Return\<^sub>e) # s\<^sub>e) \<leadsto>\<^sub>e 
-    S\<^sub>e (Const\<^sub>e n # vals_from_stack s\<^sub>c) ((map encode_closure \<Delta>, \<C>, Return\<^sub>e) # s\<^sub>e)" by simp
-  hence "iter (\<leadsto>\<^sub>e) (S\<^sub>e (vals_from_stack s\<^sub>c) ((map encode_closure \<Delta>, PushCon\<^sub>e n # \<C>, Return\<^sub>e) # s\<^sub>e)) 
-    (S\<^sub>e (Const\<^sub>e n # vals_from_stack s\<^sub>c) ((map encode_closure \<Delta>, \<C>, Return\<^sub>e) # s\<^sub>e))" 
+  then obtain \<C> s\<^sub>e where S: "stack_from_stack s\<^sub>c = (map encode_closure \<Delta>, \<C>) # s\<^sub>e" by auto
+  have "S\<^sub>e (vals_from_stack s\<^sub>c) ((map encode_closure \<Delta>, PushCon\<^sub>e n # \<C>) # s\<^sub>e) \<leadsto>\<^sub>e 
+    S\<^sub>e (Const\<^sub>e n # vals_from_stack s\<^sub>c) ((map encode_closure \<Delta>, \<C>) # s\<^sub>e)" by simp
+  hence "iter (\<leadsto>\<^sub>e) (S\<^sub>e (vals_from_stack s\<^sub>c) ((map encode_closure \<Delta>, PushCon\<^sub>e n # \<C>) # s\<^sub>e)) 
+    (S\<^sub>e (Const\<^sub>e n # vals_from_stack s\<^sub>c) ((map encode_closure \<Delta>, \<C>) # s\<^sub>e))" 
       by (metis iter_one)
   with S show ?case by simp
 next
   case (ev\<^sub>c_lam s\<^sub>c \<Delta> tt e)
   then obtain t' \<Gamma> where "(s\<^sub>c :\<^sub>c t' \<rightarrow> t) \<and> (\<Delta> :\<^sub>c\<^sub>l\<^sub>s \<Gamma>) \<and> latest_environment s\<^sub>c = Some \<Delta> \<and>
     (\<Gamma> \<turnstile>\<^sub>d Lam\<^sub>d tt e : t')" by fastforce
-  then obtain \<C> s\<^sub>e where S: "stack_from_stack s\<^sub>c = (map encode_closure \<Delta>, \<C>, Return\<^sub>e) # s\<^sub>e" by auto
-  hence "S\<^sub>e (vals_from_stack s\<^sub>c) 
-    ((map encode_closure \<Delta>, PushLam\<^sub>e (encode e) Return\<^sub>e # \<C>, Return\<^sub>e) # s\<^sub>e) \<leadsto>\<^sub>e 
-    S\<^sub>e (Lam\<^sub>e (map encode_closure \<Delta>) (encode e) Return\<^sub>e # vals_from_stack s\<^sub>c) 
-    ((map encode_closure \<Delta>, \<C>, Return\<^sub>e) # s\<^sub>e)" by (metis ev\<^sub>e_pushlam)
-  hence "iter (\<leadsto>\<^sub>e) (S\<^sub>e (vals_from_stack s\<^sub>c) 
-    ((map encode_closure \<Delta>, PushLam\<^sub>e (encode e) Return\<^sub>e # \<C>, Return\<^sub>e) # s\<^sub>e)) 
-    (S\<^sub>e (Lam\<^sub>e (map encode_closure \<Delta>) (encode e) Return\<^sub>e # vals_from_stack s\<^sub>c)
-    ((map encode_closure \<Delta>, \<C>, Return\<^sub>e) # s\<^sub>e))" by (metis iter_one)
+  then obtain \<C> s\<^sub>e where S: "stack_from_stack s\<^sub>c = (map encode_closure \<Delta>, \<C>) # s\<^sub>e" by auto
+  hence "S\<^sub>e (vals_from_stack s\<^sub>c) ((map encode_closure \<Delta>, PushLam\<^sub>e (encode e) # \<C>) # s\<^sub>e) \<leadsto>\<^sub>e 
+    S\<^sub>e (Lam\<^sub>e (map encode_closure \<Delta>) (encode e) # vals_from_stack s\<^sub>c) 
+      ((map encode_closure \<Delta>, \<C>) # s\<^sub>e)" by (metis ev\<^sub>e_pushlam)
+  hence "iter (\<leadsto>\<^sub>e) (S\<^sub>e (vals_from_stack s\<^sub>c) ((map encode_closure \<Delta>, PushLam\<^sub>e (encode e) # \<C>) # s\<^sub>e)) 
+    (S\<^sub>e (Lam\<^sub>e (map encode_closure \<Delta>) (encode e) # vals_from_stack s\<^sub>c)
+      ((map encode_closure \<Delta>, \<C>) # s\<^sub>e))" by (metis iter_one)
   with S show ?case by (simp add: encode_def)
 next
   case (ret\<^sub>c_app2 t\<^sub>1 \<Delta> e\<^sub>1 s\<^sub>c c\<^sub>2)
   then obtain \<Gamma> t\<^sub>2 \<Delta>' where "(\<Delta> :\<^sub>c\<^sub>l\<^sub>s \<Gamma>) \<and> (insert_at 0 t\<^sub>1 \<Gamma> \<turnstile>\<^sub>d e\<^sub>1 : t\<^sub>2) \<and> (s\<^sub>c :\<^sub>c t\<^sub>2 \<rightarrow> t) \<and> 
     latest_environment s\<^sub>c = Some \<Delta>' \<and> (c\<^sub>2 :\<^sub>c\<^sub>l t\<^sub>1)" by blast
-  then obtain \<C> s\<^sub>e where S: "stack_from_stack s\<^sub>c = (map encode_closure \<Delta>', \<C>, Return\<^sub>e) # s\<^sub>e" by auto
-  hence "S\<^sub>e (encode_closure c\<^sub>2 # Lam\<^sub>e (map encode_closure \<Delta>) (encode e\<^sub>1) Return\<^sub>e # 
-    vals_from_stack s\<^sub>c) ((map encode_closure \<Delta>', Apply\<^sub>e # \<C>, Return\<^sub>e) # s\<^sub>e) \<leadsto>\<^sub>e
-    S\<^sub>e (vals_from_stack s\<^sub>c) ((encode_closure c\<^sub>2 # map encode_closure \<Delta>, encode e\<^sub>1, Return\<^sub>e) # 
-    stack_from_stack s\<^sub>c)" by (metis ev\<^sub>e_apply)
-  hence "iter (\<leadsto>\<^sub>e)
-    (S\<^sub>e (encode_closure c\<^sub>2 # Lam\<^sub>e (map encode_closure \<Delta>) (encode e\<^sub>1) Return\<^sub>e # vals_from_stack s\<^sub>c) 
-    ((map encode_closure \<Delta>', Apply\<^sub>e # \<C>, Return\<^sub>e) # s\<^sub>e)) 
-    (S\<^sub>e (vals_from_stack s\<^sub>c) ((encode_closure c\<^sub>2 # map encode_closure \<Delta>, encode e\<^sub>1, Return\<^sub>e) # 
-    stack_from_stack s\<^sub>c))" by (metis iter_one)
+  then obtain \<C> s\<^sub>e where S: "stack_from_stack s\<^sub>c = (map encode_closure \<Delta>', \<C>) # s\<^sub>e" by auto
+  hence "S\<^sub>e (encode_closure c\<^sub>2 # Lam\<^sub>e (map encode_closure \<Delta>) (encode e\<^sub>1) # vals_from_stack s\<^sub>c) 
+      ((map encode_closure \<Delta>', Apply\<^sub>e # \<C>) # s\<^sub>e) \<leadsto>\<^sub>e
+    S\<^sub>e (vals_from_stack s\<^sub>c) ((encode_closure c\<^sub>2 # map encode_closure \<Delta>, encode e\<^sub>1) # 
+      stack_from_stack s\<^sub>c)" by (metis ev\<^sub>e_apply)
+  hence "iter (\<leadsto>\<^sub>e) 
+    (S\<^sub>e (encode_closure c\<^sub>2 # Lam\<^sub>e (map encode_closure \<Delta>) (encode e\<^sub>1) # vals_from_stack s\<^sub>c) 
+      ((map encode_closure \<Delta>', Apply\<^sub>e # \<C>) # s\<^sub>e)) 
+    (S\<^sub>e (vals_from_stack s\<^sub>c) ((encode_closure c\<^sub>2 # map encode_closure \<Delta>, encode e\<^sub>1) # 
+      stack_from_stack s\<^sub>c))" by (metis iter_one)
   with S show ?case by (simp add: encode_def)
 next
   case (ret\<^sub>c_ret \<Delta> s\<^sub>c c)
-  have "S\<^sub>e (encode_closure c # vals_from_stack s\<^sub>c) ((map encode_closure \<Delta>, [], Return\<^sub>e) # 
+  have "S\<^sub>e (encode_closure c # vals_from_stack s\<^sub>c) ((map encode_closure \<Delta>, [Return\<^sub>e]) # 
     stack_from_stack s\<^sub>c) \<leadsto>\<^sub>e
     S\<^sub>e (encode_closure c # vals_from_stack s\<^sub>c) (stack_from_stack s\<^sub>c)" by simp
   hence "iter (\<leadsto>\<^sub>e) 
-    (S\<^sub>e (encode_closure c # vals_from_stack s\<^sub>c) ((map encode_closure \<Delta>, [], Return\<^sub>e) # 
+    (S\<^sub>e (encode_closure c # vals_from_stack s\<^sub>c) ((map encode_closure \<Delta>, [Return\<^sub>e]) # 
     stack_from_stack s\<^sub>c))
     (S\<^sub>e (encode_closure c # vals_from_stack s\<^sub>c) (stack_from_stack s\<^sub>c))" by (metis iter_one)
   thus ?case by simp
@@ -170,7 +171,7 @@ lemma vals_from_tail_expr [simp]: "vals_from_stack (tail_expr \<Delta> e @ s\<^s
   by (induction e arbitrary: s\<^sub>c) simp_all
 
 lemma stack_from_tail_expr [simp]: "stack_from_stack (tail_expr \<Delta> e @ s\<^sub>c) = 
-    prepend_to_top_frame (tl (encode e)) (stack_from_stack s\<^sub>c)"
+    prepend_to_top_frame (tl (encode' e)) (stack_from_stack s\<^sub>c)"
   by (induction e arbitrary: s\<^sub>c) simp_all
 
 lemma evaluate_to_head_tail [simp]: "
@@ -186,139 +187,155 @@ qed simp_all
 
 text \<open>We now reconstruct encodings, stack-encodings, and state-encodings:\<close>
 
-lemma encode_not_nil [dest]: "encode e = [] \<Longrightarrow> False"
+lemma encode'_not_nil [simp]: "encode' e \<noteq> []"
   by (induction e) simp_all
 
-lemma encode_to_lookup [dest]: "encode e @ \<C>' = Lookup\<^sub>e x # \<C> \<Longrightarrow> 
-    head_expr e = Var\<^sub>d x \<and> \<C> = tl (encode e) @ \<C>'"
+lemma encode_not_nil [simp]: "encode e \<noteq> []"
+  by (simp add: encode_def)
+
+lemma encode_to_lookup [dest]: "encode' e @ \<C>' = Lookup\<^sub>e x # \<C> \<Longrightarrow> 
+    head_expr e = Var\<^sub>d x \<and> \<C> = tl (encode' e) @ \<C>'"
   by (induction e arbitrary: \<C>') fastforce+
 
-lemma encode_to_pushcon [dest]: "encode e @ \<C>' = PushCon\<^sub>e n # \<C> \<Longrightarrow> 
-    head_expr e = Const\<^sub>d n \<and> \<C> = tl (encode e) @ \<C>'"
+lemma encode_to_pushcon [dest]: "encode' e @ \<C>' = PushCon\<^sub>e n # \<C> \<Longrightarrow> 
+    head_expr e = Const\<^sub>d n \<and> \<C> = tl (encode' e) @ \<C>'"
   by (induction e arbitrary: \<C>') fastforce+
 
-lemma encode_to_pushlam [dest]: "encode e @ \<C>' = PushLam\<^sub>e \<C>'' r # \<C> \<Longrightarrow> 
-    \<exists>t e'. head_expr e = Lam\<^sub>d t e' \<and> \<C>'' = encode e' \<and> \<C> = tl (encode e) @ \<C>' \<and> r = Return\<^sub>e"
-  by (induction e arbitrary: \<C>') fastforce+
+lemma encode_to_pushlam [dest]: "encode' e @ \<C>' = PushLam\<^sub>e \<C>'' # \<C> \<Longrightarrow> 
+    \<exists>t e'. head_expr e = Lam\<^sub>d t e' \<and> \<C>'' = encode e' \<and> \<C> = tl (encode' e) @ \<C>'"
+  using encode_def by (induction e arbitrary: \<C>') fastforce+
 
-lemma encode_to_apply [dest]: "encode e @ \<C>' = Apply\<^sub>e # \<C> \<Longrightarrow> False"
+lemma encode_to_apply [dest]: "encode' e @ \<C>' = Apply\<^sub>e # \<C> \<Longrightarrow> False"
   by (induction e arbitrary: \<C>') simp_all
 
-lemma encode_lam_closure [dest]: "Lam\<^sub>e env \<C> r = encode_closure c \<Longrightarrow> 
-    \<exists>t \<Delta> e. c = Lam\<^sub>c t \<Delta> e \<and> env = map encode_closure \<Delta> \<and> \<C> = encode e \<and> r = Return\<^sub>e"
+lemma encode_to_return [dest]: "encode' e @ \<C>' = Return\<^sub>e # \<C> \<Longrightarrow> False"
+  by (induction e arbitrary: \<C>') simp_all
+
+lemma encode_to_jump [dest]: "encode' e @ \<C>' = Jump\<^sub>e # \<C> \<Longrightarrow> False"
+  by (induction e arbitrary: \<C>') simp_all
+
+lemma encode_lam_closure [dest]: "Lam\<^sub>e env \<C> = encode_closure c \<Longrightarrow> 
+    \<exists>t \<Delta> e. c = Lam\<^sub>c t \<Delta> e \<and> env = map encode_closure \<Delta> \<and> \<C> = encode e"
   by (induction c) simp_all
 
-lemma prepend_to_cons [dest]: "prepend_to_top_frame \<C>' s\<^sub>e = (\<Delta>, \<C>, r) # s\<^sub>e' \<Longrightarrow> 
-    \<exists>\<C>''. s\<^sub>e = (\<Delta>, \<C>'', r) # s\<^sub>e' \<and> \<C> = \<C>' @ \<C>''"
+lemma prepend_to_cons [dest]: "prepend_to_top_frame \<C>' s\<^sub>e = (\<Delta>, \<C>) # s\<^sub>e' \<Longrightarrow> 
+    \<exists>\<C>''. s\<^sub>e = (\<Delta>, \<C>'') # s\<^sub>e' \<and> \<C> = \<C>' @ \<C>''"
   by (induction \<C>' s\<^sub>e rule: prepend_to_top_frame.induct) simp_all
 
-lemma prepend_to_apply [dest]: "prepend_to_top_frame (encode e) s\<^sub>e = (\<Delta>, Apply\<^sub>e # \<C>, r) # s\<^sub>e' \<Longrightarrow> 
+lemma prepend_to_apply [dest]: "prepend_to_top_frame (encode' e) s\<^sub>e = (\<Delta>, Apply\<^sub>e # \<C>) # s\<^sub>e' \<Longrightarrow> 
     False"
-  by (induction "encode e" s\<^sub>e rule: prepend_to_top_frame.induct) auto
+  by (induction "encode' e" s\<^sub>e rule: prepend_to_top_frame.induct) auto
 
-lemma encode_stack_to_lookup [dest]: "stack_from_stack s\<^sub>c = (\<Delta>\<^sub>e, Lookup\<^sub>e x # \<C>, r) # s\<^sub>e \<Longrightarrow> 
-  \<exists>\<Delta>\<^sub>c e s\<^sub>c' \<C>'. s\<^sub>c = FApp1\<^sub>c \<Delta>\<^sub>c e # s\<^sub>c' \<and> stack_from_stack s\<^sub>c' = (\<Delta>\<^sub>e, \<C>', r) # s\<^sub>e \<and> 
-    head_expr e = Var\<^sub>d x \<and> \<C> = tl (encode e) @ Apply\<^sub>e # \<C>'"
+lemma prepend_to_return [dest]: "prepend_to_top_frame (encode' e) s\<^sub>e = (\<Delta>, Return\<^sub>e # \<C>) # s\<^sub>e' \<Longrightarrow> 
+    False"
+  by (induction "encode' e" s\<^sub>e rule: prepend_to_top_frame.induct) auto
+
+lemma prepend_to_jump [dest]: "prepend_to_top_frame (encode' e) s\<^sub>e = (\<Delta>, Jump\<^sub>e # \<C>) # s\<^sub>e' \<Longrightarrow> 
+    False"
+  by (induction "encode' e" s\<^sub>e rule: prepend_to_top_frame.induct) auto
+
+lemma encode_stack_to_lookup [dest]: "stack_from_stack s\<^sub>c = (\<Delta>\<^sub>e, Lookup\<^sub>e x # \<C>) # s\<^sub>e \<Longrightarrow> 
+  \<exists>\<Delta>\<^sub>c e s\<^sub>c' \<C>'. s\<^sub>c = FApp1\<^sub>c \<Delta>\<^sub>c e # s\<^sub>c' \<and> stack_from_stack s\<^sub>c' = (\<Delta>\<^sub>e, \<C>') # s\<^sub>e \<and> 
+    head_expr e = Var\<^sub>d x \<and> \<C> = tl (encode' e) @ Apply\<^sub>e # \<C>'"
 proof (induction s\<^sub>c rule: stack_from_stack.induct)
   case (2 \<Delta> e s\<^sub>c)
-  then obtain \<C>' where "stack_from_stack s\<^sub>c = (\<Delta>\<^sub>e, \<C>', r) # s\<^sub>e \<and> 
-    encode e @ Apply\<^sub>e # \<C>' = Lookup\<^sub>e x # \<C>" by fastforce
+  then obtain \<C>' where "stack_from_stack s\<^sub>c = (\<Delta>\<^sub>e, \<C>') # s\<^sub>e \<and> 
+    encode' e @ Apply\<^sub>e # \<C>' = Lookup\<^sub>e x # \<C>" by fastforce
   thus ?case by auto
 qed auto
 
-lemma encode_stack_to_pushcon [dest]: "stack_from_stack s\<^sub>c = (\<Delta>\<^sub>e, PushCon\<^sub>e n # \<C>, r) # s\<^sub>e \<Longrightarrow> 
-  \<exists>\<Delta>\<^sub>c e s\<^sub>c' \<C>'. s\<^sub>c = FApp1\<^sub>c \<Delta>\<^sub>c e # s\<^sub>c' \<and> stack_from_stack s\<^sub>c' = (\<Delta>\<^sub>e, \<C>', r) # s\<^sub>e \<and> 
-    head_expr e = Const\<^sub>d n \<and> \<C> = tl (encode e) @ Apply\<^sub>e # \<C>'"
+lemma encode_stack_to_pushcon [dest]: "stack_from_stack s\<^sub>c = (\<Delta>\<^sub>e, PushCon\<^sub>e n # \<C>) # s\<^sub>e \<Longrightarrow> 
+  \<exists>\<Delta>\<^sub>c e s\<^sub>c' \<C>'. s\<^sub>c = FApp1\<^sub>c \<Delta>\<^sub>c e # s\<^sub>c' \<and> stack_from_stack s\<^sub>c' = (\<Delta>\<^sub>e, \<C>') # s\<^sub>e \<and> 
+    head_expr e = Const\<^sub>d n \<and> \<C> = tl (encode' e) @ Apply\<^sub>e # \<C>'"
 proof (induction s\<^sub>c rule: stack_from_stack.induct)
   case (2 \<Delta>\<^sub>s e s\<^sub>c)
-  then obtain \<C>' where "stack_from_stack s\<^sub>c = (\<Delta>\<^sub>e, \<C>', r) # s\<^sub>e \<and> 
-    encode e @ Apply\<^sub>e # \<C>' = PushCon\<^sub>e n # \<C>" by fastforce
+  then obtain \<C>' where "stack_from_stack s\<^sub>c = (\<Delta>\<^sub>e, \<C>') # s\<^sub>e \<and> 
+    encode' e @ Apply\<^sub>e # \<C>' = PushCon\<^sub>e n # \<C>" by fastforce
   thus ?case by auto
 qed auto
 
-lemma encode_stack_to_pushlam [dest]: "stack_from_stack s\<^sub>c = (\<Delta>\<^sub>e, PushLam\<^sub>e \<C>' r' # \<C>, r) # s\<^sub>e \<Longrightarrow> 
-  \<exists>\<Delta>\<^sub>c e s\<^sub>c' t e' \<C>''. s\<^sub>c = FApp1\<^sub>c \<Delta>\<^sub>c e # s\<^sub>c' \<and> stack_from_stack s\<^sub>c' = (\<Delta>\<^sub>e, \<C>'', r) # s\<^sub>e \<and> 
-    head_expr e = Lam\<^sub>d t e' \<and> \<C> = tl (encode e) @ Apply\<^sub>e # \<C>'' \<and> \<C>' = encode e' \<and> r' = Return\<^sub>e"
+lemma encode_stack_to_pushlam [dest]: "stack_from_stack s\<^sub>c = (\<Delta>\<^sub>e, PushLam\<^sub>e \<C>' # \<C>) # s\<^sub>e \<Longrightarrow> 
+  \<exists>\<Delta>\<^sub>c e s\<^sub>c' t e' \<C>''. s\<^sub>c = FApp1\<^sub>c \<Delta>\<^sub>c e # s\<^sub>c' \<and> stack_from_stack s\<^sub>c' = (\<Delta>\<^sub>e, \<C>'') # s\<^sub>e \<and> 
+    head_expr e = Lam\<^sub>d t e' \<and> \<C> = tl (encode' e) @ Apply\<^sub>e # \<C>'' \<and> \<C>' = encode e'"
 proof (induction s\<^sub>c rule: stack_from_stack.induct)
   case (2 \<Delta>\<^sub>c e s\<^sub>c)
-  then obtain \<C>'' where "stack_from_stack s\<^sub>c = (\<Delta>\<^sub>e, \<C>'', r) # s\<^sub>e \<and> 
-    encode e @ Apply\<^sub>e # \<C>'' = PushLam\<^sub>e \<C>' r' # \<C>" by fastforce
+  then obtain \<C>'' where "stack_from_stack s\<^sub>c = (\<Delta>\<^sub>e, \<C>'') # s\<^sub>e \<and> 
+    encode' e @ Apply\<^sub>e # \<C>'' = PushLam\<^sub>e \<C>' # \<C>" by fastforce
   moreover then obtain t e' where "head_expr e = Lam\<^sub>d t e' \<and> \<C>' = encode e' \<and> 
-    \<C> = tl (encode e) @ Apply\<^sub>e # \<C>'' \<and> r' = Return\<^sub>e" by (metis encode_to_pushlam)
+    \<C> = tl (encode' e) @ Apply\<^sub>e # \<C>''" by (metis encode_to_pushlam)
   ultimately show ?case by auto
 qed auto
 
-lemma encode_stack_to_apply [dest]: "stack_from_stack s = (\<Delta>\<^sub>e, Apply\<^sub>e # \<C>, r) # s\<^sub>e \<Longrightarrow> 
-    \<exists>s\<^sub>c' c. s = FApp2\<^sub>c c # s\<^sub>c' \<and> stack_from_stack s\<^sub>c' = (\<Delta>\<^sub>e, \<C>, r) # s\<^sub>e"
-proof (induction s rule: stack_from_stack.induct)
-  case (3 c s\<^sub>c)
-  then show ?case by auto
-qed auto
+lemma encode_stack_to_apply [dest]: "stack_from_stack s = (\<Delta>\<^sub>e, Apply\<^sub>e # \<C>) # s\<^sub>e \<Longrightarrow> 
+    \<exists>s\<^sub>c' c. s = FApp2\<^sub>c c # s\<^sub>c' \<and> stack_from_stack s\<^sub>c' = (\<Delta>\<^sub>e, \<C>) # s\<^sub>e"
+  by (induction s rule: stack_from_stack.induct) auto
 
-lemma encode_stack_to_return [dest]: "stack_from_stack s = (\<Delta>\<^sub>e, [], r) # s\<^sub>e \<Longrightarrow> 
+lemma encode_stack_to_return [dest]: "stack_from_stack s = (\<Delta>\<^sub>e, Return\<^sub>e # \<C>) # s\<^sub>e \<Longrightarrow> 
   \<exists>\<Delta>\<^sub>c s\<^sub>c'. s = FReturn\<^sub>c \<Delta>\<^sub>c # s\<^sub>c' \<and> \<Delta>\<^sub>e = map encode_closure \<Delta>\<^sub>c \<and> s\<^sub>e = stack_from_stack s\<^sub>c' \<and> 
-    r = Return\<^sub>e"
+    \<C> = []"
+  by (induction s rule: stack_from_stack.induct) auto
+
+lemma encode_stack_to_jump [dest]: "stack_from_stack s = (\<Delta>\<^sub>e, Jump\<^sub>e # \<C>) # s\<^sub>e \<Longrightarrow> False"
   by (induction s rule: stack_from_stack.induct) auto
 
 lemma encode_state_to_lookup [dest, consumes 1, case_names SE\<^sub>c SC\<^sub>c]: "
-  encode_state \<Sigma>\<^sub>c = S\<^sub>e \<V> ((\<Delta>\<^sub>e, Lookup\<^sub>e x # \<C>, r) # s\<^sub>e) \<Longrightarrow> 
-    (\<And>s\<^sub>c \<Delta>\<^sub>c e \<C>'. head_expr e = Var\<^sub>d x \<Longrightarrow> \<C> = tl (encode e) @ \<C>' \<Longrightarrow> 
-      stack_from_stack s\<^sub>c = ((\<Delta>\<^sub>e, \<C>', r) # s\<^sub>e) \<Longrightarrow> \<V> = vals_from_stack s\<^sub>c \<Longrightarrow> P (SE\<^sub>c s\<^sub>c \<Delta>\<^sub>c e)) \<Longrightarrow> 
-    (\<And>s\<^sub>c c \<Delta>\<^sub>c e \<C>'. head_expr e = Var\<^sub>d x \<Longrightarrow> \<C> = tl (encode e) @ Apply\<^sub>e # \<C>' \<Longrightarrow> 
-      stack_from_stack s\<^sub>c = ((\<Delta>\<^sub>e, \<C>', r) # s\<^sub>e) \<Longrightarrow> \<V> = encode_closure c # vals_from_stack s\<^sub>c \<Longrightarrow> 
+  encode_state \<Sigma>\<^sub>c = S\<^sub>e \<V> ((\<Delta>\<^sub>e, Lookup\<^sub>e x # \<C>) # s\<^sub>e) \<Longrightarrow> 
+    (\<And>s\<^sub>c \<Delta>\<^sub>c e \<C>'. head_expr e = Var\<^sub>d x \<Longrightarrow> \<C> = tl (encode' e) @ \<C>' \<Longrightarrow> 
+      stack_from_stack s\<^sub>c = ((\<Delta>\<^sub>e, \<C>') # s\<^sub>e) \<Longrightarrow> \<V> = vals_from_stack s\<^sub>c \<Longrightarrow> P (SE\<^sub>c s\<^sub>c \<Delta>\<^sub>c e)) \<Longrightarrow> 
+    (\<And>s\<^sub>c c \<Delta>\<^sub>c e \<C>'. head_expr e = Var\<^sub>d x \<Longrightarrow> \<C> = tl (encode' e) @ Apply\<^sub>e # \<C>' \<Longrightarrow> 
+      stack_from_stack s\<^sub>c = ((\<Delta>\<^sub>e, \<C>') # s\<^sub>e) \<Longrightarrow> \<V> = encode_closure c # vals_from_stack s\<^sub>c \<Longrightarrow> 
       P (SC\<^sub>c (FApp1\<^sub>c \<Delta>\<^sub>c e # s\<^sub>c) c)) \<Longrightarrow> P \<Sigma>\<^sub>c"
 proof (induction \<Sigma>\<^sub>c)
   case (SE\<^sub>c s \<Delta> e)
-  moreover then obtain \<C>' where "stack_from_stack s = (\<Delta>\<^sub>e, \<C>', r) # s\<^sub>e \<and> 
-    encode e @ \<C>' = Lookup\<^sub>e x # \<C>" by auto
+  moreover then obtain \<C>' where "stack_from_stack s = (\<Delta>\<^sub>e, \<C>') # s\<^sub>e \<and> 
+    encode' e @ \<C>' = Lookup\<^sub>e x # \<C>" by auto
   ultimately show ?case by auto
 qed auto
 
 lemma encode_state_to_pushcon [dest, consumes 1, case_names SE\<^sub>c SC\<^sub>c]: "
-  encode_state \<Sigma>\<^sub>c = S\<^sub>e \<V> ((\<Delta>\<^sub>e, PushCon\<^sub>e n # \<C>, r) # s\<^sub>e) \<Longrightarrow> 
-    (\<And>s\<^sub>c \<Delta>\<^sub>c e \<C>'. head_expr e = Const\<^sub>d n \<Longrightarrow> \<C> = tl (encode e) @ \<C>' \<Longrightarrow> 
-      stack_from_stack s\<^sub>c = ((\<Delta>\<^sub>e, \<C>', r) # s\<^sub>e) \<Longrightarrow> \<V> = vals_from_stack s\<^sub>c \<Longrightarrow> P (SE\<^sub>c s\<^sub>c \<Delta>\<^sub>c e)) \<Longrightarrow> 
-    (\<And>s\<^sub>c c \<Delta>\<^sub>c e \<C>'. head_expr e = Const\<^sub>d n \<Longrightarrow> \<C> = tl (encode e) @ Apply\<^sub>e # \<C>' \<Longrightarrow> 
-      stack_from_stack s\<^sub>c = ((\<Delta>\<^sub>e, \<C>', r) # s\<^sub>e) \<Longrightarrow> \<V> = encode_closure c # vals_from_stack s\<^sub>c \<Longrightarrow> 
+  encode_state \<Sigma>\<^sub>c = S\<^sub>e \<V> ((\<Delta>\<^sub>e, PushCon\<^sub>e n # \<C>) # s\<^sub>e) \<Longrightarrow> 
+    (\<And>s\<^sub>c \<Delta>\<^sub>c e \<C>'. head_expr e = Const\<^sub>d n \<Longrightarrow> \<C> = tl (encode' e) @ \<C>' \<Longrightarrow> 
+      stack_from_stack s\<^sub>c = ((\<Delta>\<^sub>e, \<C>') # s\<^sub>e) \<Longrightarrow> \<V> = vals_from_stack s\<^sub>c \<Longrightarrow> P (SE\<^sub>c s\<^sub>c \<Delta>\<^sub>c e)) \<Longrightarrow> 
+    (\<And>s\<^sub>c c \<Delta>\<^sub>c e \<C>'. head_expr e = Const\<^sub>d n \<Longrightarrow> \<C> = tl (encode' e) @ Apply\<^sub>e # \<C>' \<Longrightarrow> 
+      stack_from_stack s\<^sub>c = ((\<Delta>\<^sub>e, \<C>') # s\<^sub>e) \<Longrightarrow> \<V> = encode_closure c # vals_from_stack s\<^sub>c \<Longrightarrow> 
       P (SC\<^sub>c (FApp1\<^sub>c \<Delta>\<^sub>c e # s\<^sub>c) c)) \<Longrightarrow> P \<Sigma>\<^sub>c"
 proof (induction \<Sigma>\<^sub>c)
   case (SE\<^sub>c s \<Delta> e)
-  moreover then obtain \<C>' where "stack_from_stack s = (\<Delta>\<^sub>e, \<C>', r) # s\<^sub>e \<and> 
-    encode e @ \<C>' = PushCon\<^sub>e n # \<C>" by auto
+  moreover then obtain \<C>' where "stack_from_stack s = (\<Delta>\<^sub>e, \<C>') # s\<^sub>e \<and> 
+    encode' e @ \<C>' = PushCon\<^sub>e n # \<C>" by auto
   ultimately show ?case by auto
 qed auto
 
 lemma encode_state_to_pushlam [dest, consumes 1, case_names SE\<^sub>c SC\<^sub>c]: "
-  encode_state \<Sigma>\<^sub>c = S\<^sub>e \<V> ((\<Delta>\<^sub>e, PushLam\<^sub>e \<C>' r' # \<C>, r) # s\<^sub>e) \<Longrightarrow> 
+  encode_state \<Sigma>\<^sub>c = S\<^sub>e \<V> ((\<Delta>\<^sub>e, PushLam\<^sub>e \<C>' # \<C>) # s\<^sub>e) \<Longrightarrow> 
     (\<And>s\<^sub>c \<Delta>\<^sub>c e tt e' \<C>''. \<Sigma>\<^sub>c = SE\<^sub>c s\<^sub>c \<Delta>\<^sub>c e \<Longrightarrow> head_expr e = Lam\<^sub>d tt e' \<Longrightarrow> 
-      \<C> = tl (encode e) @ \<C>'' \<Longrightarrow> \<C>' = encode e' \<Longrightarrow> \<V> = vals_from_stack s\<^sub>c \<Longrightarrow> 
-      stack_from_stack s\<^sub>c = (\<Delta>\<^sub>e, \<C>'', r) # s\<^sub>e \<Longrightarrow> r' = Return\<^sub>e \<Longrightarrow> P) \<Longrightarrow> 
+      \<C> = tl (encode' e) @ \<C>'' \<Longrightarrow> \<C>' = encode e' \<Longrightarrow> \<V> = vals_from_stack s\<^sub>c \<Longrightarrow> 
+      stack_from_stack s\<^sub>c = (\<Delta>\<^sub>e, \<C>'') # s\<^sub>e \<Longrightarrow> P) \<Longrightarrow> 
     (\<And>s\<^sub>c c \<Delta>\<^sub>c e tt e' \<C>''. \<Sigma>\<^sub>c = SC\<^sub>c (FApp1\<^sub>c \<Delta>\<^sub>c e # s\<^sub>c) c \<Longrightarrow> head_expr e = Lam\<^sub>d tt e' \<Longrightarrow> 
-      \<C> = tl (encode e) @ Apply\<^sub>e # \<C>'' \<Longrightarrow> \<C>' = encode e' \<Longrightarrow> 
-      \<V> = encode_closure c # vals_from_stack s\<^sub>c \<Longrightarrow> stack_from_stack s\<^sub>c = (\<Delta>\<^sub>e, \<C>'', r) # s\<^sub>e \<Longrightarrow> 
-      r' = Return\<^sub>e \<Longrightarrow> P) \<Longrightarrow> 
+      \<C> = tl (encode' e) @ Apply\<^sub>e # \<C>'' \<Longrightarrow> \<C>' = encode e' \<Longrightarrow> 
+      \<V> = encode_closure c # vals_from_stack s\<^sub>c \<Longrightarrow> stack_from_stack s\<^sub>c = (\<Delta>\<^sub>e, \<C>'') # s\<^sub>e \<Longrightarrow> P) \<Longrightarrow> 
     P"
 proof (induction \<Sigma>\<^sub>c)
   case (SE\<^sub>c s\<^sub>c \<Delta>\<^sub>c e)
-  moreover then obtain \<C>'' where "stack_from_stack s\<^sub>c = (\<Delta>\<^sub>e, \<C>'', r) # s\<^sub>e \<and> 
-    encode e @ \<C>'' = PushLam\<^sub>e \<C>' r' # \<C>" by auto
+  moreover then obtain \<C>'' where "stack_from_stack s\<^sub>c = (\<Delta>\<^sub>e, \<C>'') # s\<^sub>e \<and> 
+    encode' e @ \<C>'' = PushLam\<^sub>e \<C>' # \<C>" by auto
   moreover then obtain tt e' where "head_expr e = Lam\<^sub>d tt e' \<and> \<C>' = encode e' \<and> 
-    \<C> = tl (encode e) @ \<C>'' \<and> r' = Return\<^sub>e" by (metis encode_to_pushlam)
+    \<C> = tl (encode' e) @ \<C>''" by (metis encode_to_pushlam)
   ultimately show ?case by auto
 qed auto
 
 lemma encode_state_to_apply [dest]: "
-  encode_state \<Sigma>\<^sub>c = S\<^sub>e (v # Lam\<^sub>e \<Delta>\<^sub>e' \<C>' r' # \<V>) ((\<Delta>\<^sub>e, Apply\<^sub>e # \<C>, r) # s\<^sub>e) \<Longrightarrow>
-    \<exists>s\<^sub>c c c'. \<Sigma>\<^sub>c = SC\<^sub>c (FApp2\<^sub>c c' # s\<^sub>c) c \<and> stack_from_stack s\<^sub>c = ((\<Delta>\<^sub>e, \<C>, r) # s\<^sub>e) \<and> 
-      v = encode_closure c \<and> Lam\<^sub>e \<Delta>\<^sub>e' \<C>' r' = encode_closure c' \<and> \<V> = vals_from_stack s\<^sub>c"
+  encode_state \<Sigma>\<^sub>c = S\<^sub>e (v # Lam\<^sub>e \<Delta>\<^sub>e' \<C>' # \<V>) ((\<Delta>\<^sub>e, Apply\<^sub>e # \<C>) # s\<^sub>e) \<Longrightarrow>
+    \<exists>s\<^sub>c c c'. \<Sigma>\<^sub>c = SC\<^sub>c (FApp2\<^sub>c c' # s\<^sub>c) c \<and> stack_from_stack s\<^sub>c = ((\<Delta>\<^sub>e, \<C>) # s\<^sub>e) \<and> 
+      v = encode_closure c \<and> Lam\<^sub>e \<Delta>\<^sub>e' \<C>' = encode_closure c' \<and> \<V> = vals_from_stack s\<^sub>c"
   by (induction \<Sigma>\<^sub>c) auto
 
-lemma encode_state_to_return [dest]: "encode_state \<Sigma>\<^sub>c = S\<^sub>e \<V> ((\<Delta>\<^sub>e, [], Return\<^sub>e) # s\<^sub>e) \<Longrightarrow> 
-  (\<exists>\<Delta>\<^sub>c s c. \<Sigma>\<^sub>c = SC\<^sub>c (FReturn\<^sub>c \<Delta>\<^sub>c # s) c \<and> s\<^sub>e = stack_from_stack s \<and>
-    \<Delta>\<^sub>e = map encode_closure \<Delta>\<^sub>c \<and> \<V> = encode_closure c # vals_from_stack s)"
+lemma encode_state_to_return [dest]: "encode_state \<Sigma>\<^sub>c = S\<^sub>e \<V> ((\<Delta>\<^sub>e, Return\<^sub>e # \<C>) # s\<^sub>e) \<Longrightarrow> 
+  \<exists>\<Delta>\<^sub>c s c. \<Sigma>\<^sub>c = SC\<^sub>c (FReturn\<^sub>c \<Delta>\<^sub>c # s) c \<and> s\<^sub>e = stack_from_stack s \<and>
+    \<Delta>\<^sub>e = map encode_closure \<Delta>\<^sub>c \<and> \<V> = encode_closure c # vals_from_stack s \<and> \<C> = []"
   by (induction \<Sigma>\<^sub>c) auto
 
-lemma encode_state_to_jump [dest]: "encode_state \<Sigma>\<^sub>c = S\<^sub>e \<V> ((\<Delta>\<^sub>e, [], Jump\<^sub>e) # s\<^sub>e) \<Longrightarrow> False"
+lemma encode_state_to_jump [dest]: "encode_state \<Sigma>\<^sub>c = S\<^sub>e \<V> ((\<Delta>\<^sub>e, Jump\<^sub>e # \<C>) # s\<^sub>e) \<Longrightarrow> False"
   by (induction \<Sigma>\<^sub>c) auto
 
 text \<open>And now, we can finally prove completeness.\<close>
@@ -326,8 +343,8 @@ text \<open>And now, we can finally prove completeness.\<close>
 theorem complete\<^sub>e [simp]: "encode_state \<Sigma>\<^sub>c \<leadsto>\<^sub>e \<Sigma>\<^sub>t' \<Longrightarrow> \<Sigma>\<^sub>c :\<^sub>c t \<Longrightarrow>
   \<exists>\<Sigma>\<^sub>c'. iter (\<leadsto>\<^sub>c) \<Sigma>\<^sub>c \<Sigma>\<^sub>c' \<and> \<Sigma>\<^sub>t' = encode_state \<Sigma>\<^sub>c'"
 proof (induction "encode_state \<Sigma>\<^sub>c" \<Sigma>\<^sub>t' rule: eval\<^sub>e.induct)
-  case (ev\<^sub>e_lookup \<Delta>\<^sub>e x v \<V> \<C> r s\<^sub>e)
-  hence X: "encode_state \<Sigma>\<^sub>c = S\<^sub>e \<V> ((\<Delta>\<^sub>e, Lookup\<^sub>e x # \<C>, r) # s\<^sub>e)" by simp
+  case (ev\<^sub>e_lookup \<Delta>\<^sub>e x v \<V> \<C> s\<^sub>e)
+  hence X: "encode_state \<Sigma>\<^sub>c = S\<^sub>e \<V> ((\<Delta>\<^sub>e, Lookup\<^sub>e x # \<C>) # s\<^sub>e)" by simp
   from X ev\<^sub>e_lookup(1, 3) show ?case
   proof (induction rule: encode_state_to_lookup)
     case (SE\<^sub>c s\<^sub>c \<Delta>\<^sub>c e \<C>')
@@ -348,8 +365,8 @@ proof (induction "encode_state \<Sigma>\<^sub>c" \<Sigma>\<^sub>t' rule: eval\<^
     with SC\<^sub>c C show ?case by auto
   qed
 next
-  case (ev\<^sub>e_pushcon \<V> \<Delta>\<^sub>e n \<C> r s\<^sub>e)
-  hence X: "encode_state \<Sigma>\<^sub>c = S\<^sub>e \<V> ((\<Delta>\<^sub>e, PushCon\<^sub>e n # \<C>, r) # s\<^sub>e)" by simp
+  case (ev\<^sub>e_pushcon \<V> \<Delta>\<^sub>e n \<C> s\<^sub>e)
+  hence X: "encode_state \<Sigma>\<^sub>c = S\<^sub>e \<V> ((\<Delta>\<^sub>e, PushCon\<^sub>e n # \<C>) # s\<^sub>e)" by simp
   from X ev\<^sub>e_pushcon(2) show ?case
   proof (induction rule: encode_state_to_pushcon)
     case (SE\<^sub>c s\<^sub>c \<Delta>\<^sub>c e \<C>')
@@ -369,8 +386,8 @@ next
     with SC\<^sub>c show ?case by auto
   qed
 next
-  case (ev\<^sub>e_pushlam \<V> \<Delta>\<^sub>e \<C>' r' \<C> r s\<^sub>e)
-  hence X: "encode_state \<Sigma>\<^sub>c = S\<^sub>e \<V> ((\<Delta>\<^sub>e, PushLam\<^sub>e \<C>' r' # \<C>, r) # s\<^sub>e)" by simp
+  case (ev\<^sub>e_pushlam \<V> \<Delta>\<^sub>e \<C>' \<C> s\<^sub>e)
+  hence X: "encode_state \<Sigma>\<^sub>c = S\<^sub>e \<V> ((\<Delta>\<^sub>e, PushLam\<^sub>e \<C>' # \<C>) # s\<^sub>e)" by simp
   from X ev\<^sub>e_pushlam(2) show ?case
   proof (induction rule: encode_state_to_pushlam)
     case (SE\<^sub>c s\<^sub>c \<Delta>\<^sub>c e tt e' \<C>'')
@@ -379,7 +396,7 @@ next
       SC\<^sub>c (tail_expr \<Delta>\<^sub>c e @ s\<^sub>c) (Lam\<^sub>c tt \<Delta>\<^sub>c e')" by simp
     ultimately have E: "iter (\<leadsto>\<^sub>c) (SE\<^sub>c s\<^sub>c \<Delta>\<^sub>c e) (SC\<^sub>c (tail_expr \<Delta>\<^sub>c e @ s\<^sub>c) (Lam\<^sub>c tt \<Delta>\<^sub>c e'))"
       by (metis iter_step_after)
-    from SE\<^sub>c have "\<Delta>\<^sub>e = map encode_closure \<Delta>\<^sub>c \<and> r' = Return\<^sub>e" by fastforce
+    from SE\<^sub>c have "\<Delta>\<^sub>e = map encode_closure \<Delta>\<^sub>c" by fastforce
     with SE\<^sub>c E show ?case by auto
   next
     case (SC\<^sub>c s\<^sub>c c \<Delta>\<^sub>c e tt e' \<C>'')
@@ -391,15 +408,15 @@ next
     ultimately have E: "iter (\<leadsto>\<^sub>c) (SC\<^sub>c (FApp1\<^sub>c \<Delta>\<^sub>c e # s\<^sub>c) c) 
       (SC\<^sub>c (tail_expr \<Delta>\<^sub>c e @ FApp2\<^sub>c c # s\<^sub>c) (Lam\<^sub>c tt \<Delta>\<^sub>c e'))" 
         by (metis iter_step iter_step_after)
-    from SC\<^sub>c have "\<Delta>\<^sub>e = map encode_closure \<Delta>\<^sub>c \<and> r' = Return\<^sub>e" by fastforce
+    from SC\<^sub>c have "\<Delta>\<^sub>e = map encode_closure \<Delta>\<^sub>c" by fastforce
     with SC\<^sub>c E show ?case by auto
   qed
 next
-  case (ev\<^sub>e_apply v \<Delta>\<^sub>e' \<C>' r' \<V> \<Delta>\<^sub>e \<C> r s\<^sub>e)
-  hence "encode_state \<Sigma>\<^sub>c = S\<^sub>e (v # Lam\<^sub>e \<Delta>\<^sub>e' \<C>' r' # \<V>) ((\<Delta>\<^sub>e, Apply\<^sub>e # \<C>, r) # s\<^sub>e)" by simp
+  case (ev\<^sub>e_apply v \<Delta>\<^sub>e' \<C>' \<V> \<Delta>\<^sub>e \<C> s\<^sub>e)
+  hence "encode_state \<Sigma>\<^sub>c = S\<^sub>e (v # Lam\<^sub>e \<Delta>\<^sub>e' \<C>' # \<V>) ((\<Delta>\<^sub>e, Apply\<^sub>e # \<C>) # s\<^sub>e)" by simp
   then obtain s\<^sub>c c c' where "\<Sigma>\<^sub>c = SC\<^sub>c (FApp2\<^sub>c c' # s\<^sub>c) c \<and> 
-    stack_from_stack s\<^sub>c = ((\<Delta>\<^sub>e, \<C>, r) # s\<^sub>e) \<and> v = encode_closure c \<and> 
-    Lam\<^sub>e \<Delta>\<^sub>e' \<C>' r' = encode_closure c' \<and> \<V> = vals_from_stack s\<^sub>c" 
+    stack_from_stack s\<^sub>c = ((\<Delta>\<^sub>e, \<C>) # s\<^sub>e) \<and> v = encode_closure c \<and> 
+    Lam\<^sub>e \<Delta>\<^sub>e' \<C>' = encode_closure c' \<and> \<V> = vals_from_stack s\<^sub>c" 
       by auto
   moreover then obtain t \<Delta>\<^sub>c e where "c' = Lam\<^sub>c t \<Delta>\<^sub>c e \<and> \<Delta>\<^sub>e' = map encode_closure \<Delta>\<^sub>c \<and> 
     \<C>' = encode e" by auto
@@ -407,18 +424,18 @@ next
     by simp
   moreover hence "iter (\<leadsto>\<^sub>c) (SC\<^sub>c (FApp2\<^sub>c (Lam\<^sub>c t \<Delta>\<^sub>c e) # s\<^sub>c) c) 
     (SE\<^sub>c (FReturn\<^sub>c (c # \<Delta>\<^sub>c) # s\<^sub>c) (c # \<Delta>\<^sub>c) e)" by (metis iter_one)
-  ultimately show ?case by auto
+  ultimately show ?case by (auto simp add: encode_def)
 next
-  case (ev\<^sub>e_return \<V> \<Delta>\<^sub>e s\<^sub>e)
-  hence "encode_state \<Sigma>\<^sub>c = S\<^sub>e \<V> ((\<Delta>\<^sub>e, [], Return\<^sub>e) # s\<^sub>e)" by simp
+  case (ev\<^sub>e_return \<V> \<Delta>\<^sub>e \<C> s\<^sub>e)
+  hence "encode_state \<Sigma>\<^sub>c = S\<^sub>e \<V> ((\<Delta>\<^sub>e, Return\<^sub>e # \<C>) # s\<^sub>e)" by simp
   then obtain \<Delta>\<^sub>c s\<^sub>c c where S: "\<Sigma>\<^sub>c = SC\<^sub>c (FReturn\<^sub>c \<Delta>\<^sub>c # s\<^sub>c) c \<and> s\<^sub>e = stack_from_stack s\<^sub>c \<and>
     \<Delta>\<^sub>e = map encode_closure \<Delta>\<^sub>c \<and> \<V> = encode_closure c # vals_from_stack s\<^sub>c" by auto
   have "SC\<^sub>c (FReturn\<^sub>c \<Delta>\<^sub>c # s\<^sub>c) c \<leadsto>\<^sub>c SC\<^sub>c s\<^sub>c c" by simp
   hence "iter (\<leadsto>\<^sub>c) (SC\<^sub>c (FReturn\<^sub>c \<Delta>\<^sub>c # s\<^sub>c) c) (SC\<^sub>c s\<^sub>c c)" by (metis iter_one)
   with S show ?case by auto
 next
-  case (ev\<^sub>e_jump v \<Delta>\<^sub>e' \<C>' r' \<V> \<Delta>\<^sub>e s\<^sub>e)
-  hence "encode_state \<Sigma>\<^sub>c = S\<^sub>e (v # Lam\<^sub>e \<Delta>\<^sub>e' \<C>' r' # \<V>) ((\<Delta>\<^sub>e, [], Jump\<^sub>e) # s\<^sub>e)" by simp
+  case (ev\<^sub>e_jump v \<Delta>\<^sub>e' \<C>' \<V> \<Delta>\<^sub>e \<C> s\<^sub>e)
+  hence "encode_state \<Sigma>\<^sub>c = S\<^sub>e (v # Lam\<^sub>e \<Delta>\<^sub>e' \<C>' # \<V>) ((\<Delta>\<^sub>e, Jump\<^sub>e # \<C>) # s\<^sub>e)" by simp
   thus ?case by auto
 qed
 
